theories/logic/sem_types.v
@@ -22,6 +22,7 @@ From affine_tes.logic Require Import iEff.
 From affine_tes.logic Require Import sem_def.
 
 (* Base types. *)
+Definition sem_ty_void {Σ} : sem_ty Σ := (λ v, False)%I.
 Definition sem_ty_unit {Σ} : sem_ty Σ := (λ v, ⌜ v = #() ⌝)%I.
 Definition sem_ty_bool {Σ} : sem_ty Σ := (λ v, ∃ b : bool, ⌜ v = #b ⌝)%I.
 Definition sem_ty_int {Σ} : sem_ty Σ := (λ v, ∃ n : Z, ⌜ v = #n ⌝)%I.
@@ -48,104 +49,35 @@ Definition sem_ty_sum {Σ} (τ κ : sem_ty Σ) : sem_ty Σ :=
 
 (* Affine Arrow type. *)
 Definition sem_ty_aarr `{irisGS eff_lang Σ}
-  (Γ₁ : env Σ)
-  (Γ₂ : env Σ)
-  (ρ : sem_sig Σ)
+  (ρs : sem_sigs Σ)
   (τ : sem_ty Σ)
   (κ : sem_ty Σ) : sem_ty Σ :=
   (λ (v : val),
-    ∀ (w : val) (vs : gmap string val),
-      ⟦ Γ₁ ⟧ vs -∗
+    ∀ (w : val),
       τ w -∗
-      EWP (v <_ map (subst_map vs ∘ Var) (env_dom Γ₁) _> w) <| ρ |> {{ u, κ u ∗ ⟦ Γ₂ ⟧ vs }})%I.
+      EWP (v w) <| fst ρs |> {| snd ρs |} {{ u, κ u }})%I.
 
 (* Unrestricted Arrow type. *)
 Definition sem_ty_uarr `{irisGS eff_lang Σ} 
-  (Γ₁ : env Σ)
-  (Γ₂ : env Σ)
-  (ρ : sem_sig Σ)
+  (ρs : sem_sigs Σ)
   (τ : sem_ty Σ)
   (κ : sem_ty Σ) : sem_ty Σ :=
   (λ (v : val), □ (
-    ∀ (w : val) (vs : gmap string val),
-      ⟦ Γ₁ ⟧ vs -∗ 
+    ∀ (w : val),
       τ w -∗ 
-      EWP (v <_ map (subst_map vs ∘ Var) (env_dom Γ₁) _> w) <| ρ |> {{ u, κ u ∗ ⟦ Γ₂ ⟧ vs }}))%I.
-
-(* Sequentially Unrestricted Arrow type. *)
-Definition sem_ty_suarr_pre `{irisGS eff_lang Σ} 
-  (Γ₁ : env Σ)
-  (Γ₂ : env Σ)
-  (ρ : sem_sig Σ)
-  (τ : sem_ty Σ)
-  (κ : sem_ty Σ) 
-  (rec : sem_ty Σ) : sem_ty Σ :=
-  (λ (v : val), ∀ (w : val) (vs : gmap string val),
-      ⟦ Γ₁ ⟧ vs -∗ 
-      τ w -∗ 
-      EWP (v <_ map (subst_map vs ∘ Var) (env_dom Γ₁) _> w) <| ρ |> {{ u, κ u ∗ ⟦ Γ₂ ⟧ vs ∗ rec v }})%I.
-
-Global Instance sem_ty_suarr_pre_contractive `{irisGS eff_lang Σ} 
-  (ρ : sem_sig Σ) (Γ₁ Γ₂ : env Σ) (τ κ : sem_ty Σ) :
-  Contractive (sem_ty_suarr_pre Γ₁ Γ₂ ρ τ κ).
-Proof. 
-  intros ????. unfold sem_ty_suarr_pre. intros ?.
-  do 2 (rewrite bi.forall_ne; first done; intros ?). f_equiv.
-  rewrite /ewp_def.
-  assert (Hunfold : ∀ z,
-            fixpoint ewp_pre ⊤ (app_mult x0 (map (subst_map a0 ∘ Var) (env_dom Γ₁)) a) ρ
-              iEff_bottom (λ u : val, (κ u ∗ ⟦ Γ₂ ⟧ a0 ∗ z x0)%I) ≡{n}≡ 
-            ewp_pre (fixpoint ewp_pre) ⊤ (app_mult x0 (map (subst_map a0 ∘ Var) (env_dom Γ₁)) a) ρ
-              iEff_bottom (λ u : val, (κ u ∗ ⟦ Γ₂ ⟧ a0 ∗ z x0)%I)).
-  { intros ?. apply non_dep_fun_dist5. by rewrite  -fixpoint_unfold. }
-  rewrite (Hunfold x) (Hunfold y). clear Hunfold. rewrite /ewp_pre.
-  destruct (to_val) eqn:Hval; first done. 
-  destruct (to_eff) eqn:Heff; first done. rewrite -/ewp_pre. simpl.
-  do 22 (f_contractive || f_equiv).
-  induction num_laters_per_step as [|k IHk]; simpl; last (by rewrite IHk).
-  do 2 f_equiv. rewrite -/ewp_def.
-  do 2 f_equiv. intros ?. do 2 f_equiv. by apply non_dep_fun_dist.
-Qed.
-
-Definition sem_ty_suarr `{irisGS eff_lang Σ}
-  (Γ₁ Γ₂ : env Σ)
-  (ρ : sem_sig Σ)
-  (τ : sem_ty Σ)
-  (κ : sem_ty Σ) : sem_ty Σ := fixpoint (sem_ty_suarr_pre Γ₁ Γ₂ ρ τ κ).
-
-Lemma sem_ty_suarr_unfold `{irisGS eff_lang Σ}
-  (Γ₁ Γ₂ : env Σ)
-  (ρ : sem_sig Σ)
-  (τ : sem_ty Σ)
-  (κ : sem_ty Σ) 
-  (v : val) :
-  (sem_ty_suarr Γ₁ Γ₂ ρ τ κ)%V v ⊣⊢
-    (∀ (w : val) (vs : gmap string val),
-      ⟦ Γ₁ ⟧ vs -∗ 
-      τ w -∗ 
-      EWP (v <_ map (subst_map vs ∘ Var) (env_dom Γ₁) _>  w) <| ρ |> {{ u, κ u ∗ 
-                                                                           ⟦ Γ₂ ⟧ vs ∗ 
-                                                                           sem_ty_suarr Γ₁ Γ₂ ρ τ κ v }})%I.
-Proof.
-  unfold sem_ty_suarr. 
-  set suarr := sem_ty_suarr_pre Γ₁ Γ₂ ρ τ κ.
-  assert (Hfix : fixpoint suarr v ≡ suarr (fixpoint suarr) v).
-  { iApply non_dep_fun_equiv. apply fixpoint_unfold. }
-  etrans; [apply Hfix|].
-  by rewrite /sem_ty_suarr_pre.
-Qed.
+      EWP (v w) <| fst ρs |> {| snd ρs |} {{ u, κ u }}))%I.
 
 (* Polymorphic type. *)
 Definition sem_ty_forall `{irisGS eff_lang Σ} 
-  (ρ : sem_sig Σ) (C : sem_ty Σ → sem_ty Σ) : sem_ty Σ := 
-    (λ v, ∀ τ, □ EWP (v <_>) <| ρ |> {{ C τ }})%I.
+  (ρs : sem_sigs Σ) (C : sem_ty Σ → sem_ty Σ) : sem_ty Σ := 
+    (λ v, ∀ τ, □ EWP (v <_>) <| fst ρs |> {| snd ρs |} {{ C τ }})%I.
 
 (* Polymorphic effect type. *)
 (* why is value restriction also important here? *)
 (* example: ∀ θ, ∀ τ, (τ -{ θ }-> ()) -{ θ }-> () *)
 Definition sem_ty_sig_forall `{irisGS eff_lang Σ} 
-  (τ : sem_sig Σ → sem_ty Σ) : sem_ty Σ := 
-    (λ v, ∀ θ, EWP (v <_>) <| θ |> {{ τ θ }})%I.
+  (τ : sem_sigs Σ → sem_ty Σ) : sem_ty Σ := 
+    (λ v, ∀ θ, EWP (v <_>) <| fst θ |> {| snd θ |} {{ τ θ }})%I.
 
 (* Existential type. *)
 Definition sem_ty_exists `{irisGS eff_lang Σ} 
@@ -182,98 +114,126 @@ Definition sem_sig_nil {Σ} : sem_sig Σ := iEff_bottom.
 
 (* Universally Quantified, Recursive Effect Signature *)
 
-(* Effect Signature *)
-Definition sem_sig_eff_rec_pre {Σ} (A B : sem_ty Σ -d> sem_sig Σ -d> sem_ty Σ) (rec : sem_sig Σ) : sem_sig Σ :=
-  (>> (α : sem_ty Σ) (a : val) >> ! a {{ ▷ (∃ rec', rec ≡ rec' ∧ A α rec' a) }}; 
-   << (b : val)                << ? b {{ ▷ (∃ rec', rec ≡ rec' ∧ B α rec' b) }} @OS).
+Definition select_m (m : mode) (v : val) := 
+  match m with
+    OS => InjLV v
+  | MS => InjRV v
+  end.
 
-Global Instance sem_sig_eff_rec_pre_contractive {Σ} (A B : sem_ty Σ -d> sem_sig Σ -d> sem_ty Σ) :
-  Contractive (sem_sig_eff_rec_pre A B).
+(* Effect Signature *)
+Definition sem_sig_eff_rec_pre {Σ} m (A B : sem_ty Σ -d> sem_sig Σ -d> sem_ty Σ) (rec : sem_sig Σ) : sem_sig Σ :=
+  (>> (α : sem_ty Σ) (a : val) >> ! (select_m m a) {{ ▷ (∃ rec', rec ≡ rec' ∧ A α rec' a) }}; 
+   << (b : val)                << ? b {{ ▷ (∃ rec', rec ≡ rec' ∧ B α rec' b) }} @m).
+
+Global Instance sem_sig_eff_rec_pre_contractive {Σ} m (A B : sem_ty Σ -d> sem_sig Σ -d> sem_ty Σ) :
+  Contractive (sem_sig_eff_rec_pre m A B).
 Proof.
   intros ?????. 
   rewrite /sem_sig_eff_rec_pre iEffPre_exist_eq iEffPost_exist_eq /=.
   intros ?. simpl. do 3 f_equiv. rewrite iEffPre_base_eq /=.
   intros ?. simpl. do 2 f_equiv.
   { f_contractive. simpl in H. by do 4 f_equiv. }
-  f_equiv. intros ?. rewrite /iEffPost_exist_def. do 3 f_equiv.
+  do 2 f_equiv. intros ?. rewrite /iEffPost_exist_def. do 3 f_equiv.
   rewrite iEffPost_base_eq /iEffPost_base_def. f_equiv. f_contractive.
   simpl in H. by do 4 f_equiv.
 Qed.
 
-Definition sem_sig_eff_rec {Σ} (A B : sem_ty Σ → sem_sig Σ → sem_ty Σ) : sem_sig Σ :=
-  fixpoint (sem_sig_eff_rec_pre A B).
+Definition sem_sig_eff_rec {Σ} m (A B : sem_ty Σ → sem_sig Σ → sem_ty Σ) : sem_sig Σ :=
+  fixpoint (sem_sig_eff_rec_pre m A B).
 
-Lemma sem_sig_eff_rec_unfold {Σ} (A B : sem_ty Σ → sem_sig Σ → sem_ty Σ) `{NonExpansive2 A, NonExpansive2 B} :
-  (sem_sig_eff_rec A B) ≡ 
-    (>> (α : sem_ty Σ) (a : val) >> ! a {{ ▷ (A α (sem_sig_eff_rec A B) a) }}; 
-     << (b : val)                << ? b {{ ▷ (B α (sem_sig_eff_rec A B) b) }} @OS)%ieff.
+Lemma sem_sig_eff_rec_unfold {Σ} m (A B : sem_ty Σ → sem_sig Σ → sem_ty Σ) `{NonExpansive2 A, NonExpansive2 B} :
+  (sem_sig_eff_rec m A B) ≡ 
+    (>> (α : sem_ty Σ) (a : val) >> ! (select_m m a) {{ ▷ (A α (sem_sig_eff_rec m A B) a) }}; 
+     << (b : val)                << ? b {{ ▷ (B α (sem_sig_eff_rec m A B) b) }} @m)%ieff.
 Proof.
   rewrite {1} /sem_sig_eff_rec fixpoint_unfold {1} /sem_sig_eff_rec_pre.
   do 5 f_equiv. 
   - iSplit. 
     + iIntros "[% [#Hfix HA]] !>". 
       rewrite /sem_sig_eff_rec.
-      iAssert (A a rec' ≡ A a (fixpoint (sem_sig_eff_rec_pre A B)))%I as "#H".
+      iAssert (A a rec' ≡ A a (fixpoint (sem_sig_eff_rec_pre m A B)))%I as "#H".
       { by iRewrite "Hfix". }
       rewrite discrete_fun_equivI. by iRewrite - ("H" $! a0).
-    + iIntros "HA //=". iExists (sem_sig_eff_rec A B).
+    + iIntros "HA //=". iExists (sem_sig_eff_rec m A B).
       by iFrame. 
   - intros ?. rewrite iEffPost_base_eq /iEffPost_base_def.
     apply non_dep_fun_equiv. do 2 f_equiv. intros ?. do 2 f_equiv. iSplit.
     + iIntros "[% [#Hfix HB]]". 
       rewrite /sem_sig_eff_rec.
-      iAssert (B a rec' ≡ B a (fixpoint (sem_sig_eff_rec_pre A B)))%I as "#H".
+      iAssert (B a rec' ≡ B a (fixpoint (sem_sig_eff_rec_pre m A B)))%I as "#H".
       { by iRewrite "Hfix". }
       rewrite discrete_fun_equivI. by iRewrite - ("H" $! a1).
-    + iIntros "Hτ //=". iExists (sem_sig_eff_rec A B).
+    + iIntros "Hτ //=". iExists (sem_sig_eff_rec m A B).
       by iFrame. 
 Qed.
 
-Lemma sem_sig_eff_rec_unfold' {Σ} (A B : sem_ty Σ -d> sem_sig Σ -d> sem_ty Σ) `{ NonExpansive2 A, NonExpansive2 B } v Φ:
-  iEff_car (sem_sig_eff_rec A B) v Φ ⊣⊢
-    iEff_car (>> (α : sem_ty Σ) (a : val) >> ! a {{ ▷ (A α (sem_sig_eff_rec A B) a) }}; 
-              << (b : val)                << ? b {{ ▷ (B α (sem_sig_eff_rec A B) b) }} @OS)%ieff v Φ.
+Lemma sem_sig_eff_rec_unfold' {Σ} m (A B : sem_ty Σ -d> sem_sig Σ -d> sem_ty Σ) `{ NonExpansive2 A, NonExpansive2 B } v Φ:
+  iEff_car (sem_sig_eff_rec m A B) v Φ ⊣⊢
+    iEff_car (>> (α : sem_ty Σ) (a : val) >> ! (select_m m a) {{ ▷ (A α (sem_sig_eff_rec m A B) a) }}; 
+              << (b : val)                << ? b {{ ▷ (B α (sem_sig_eff_rec m A B) b) }} @m)%ieff v Φ.
 Proof.
   assert (Hequiv :
-  iEff_car (sem_sig_eff_rec A B) v Φ ⊣⊢
-    iEff_car (>> (α : sem_ty Σ) (a : val) >> ! a {{ ▷ (A α (sem_sig_eff_rec A B) a) }}; 
-              << (b : val)                << ? b {{ ▷ (B α (sem_sig_eff_rec A B) b) }} @OS)%ieff v Φ).
+  iEff_car (sem_sig_eff_rec m A B) v Φ ⊣⊢
+    iEff_car (>> (α : sem_ty Σ) (a : val) >> ! (select_m m a) {{ ▷ (A α (sem_sig_eff_rec m A B) a) }}; 
+              << (b : val)                << ? b {{ ▷ (B α (sem_sig_eff_rec m A B) b) }} @m)%ieff v Φ).
   { f_equiv. apply non_dep_fun_equiv. by apply sem_sig_eff_rec_unfold. }
   by rewrite Hequiv.
 Qed.
 
-Lemma sem_sig_eff_rec_eq {Σ} A B v Φ `{ NonExpansive2 A, NonExpansive2 B }:
-  iEff_car (sem_sig_eff_rec (Σ:=Σ) A B) v Φ ⊣⊢
-    (∃ α a, ⌜ a = v ⌝ ∗ (▷ A α (sem_sig_eff_rec A B) a) ∗ 
-                        (∀ b, (▷ B α (sem_sig_eff_rec A B) b) -∗ Φ b))%I.
+Lemma sem_sig_eff_rec_eq {Σ} m A B v Φ `{ NonExpansive2 A, NonExpansive2 B }:
+  iEff_car (sem_sig_eff_rec (Σ:=Σ) m A B) v Φ ⊣⊢
+    (∃ α a, ⌜ (select_m m a) = v ⌝ ∗ (▷ A α (sem_sig_eff_rec m A B) a) ∗ 
+                        □? m (∀ b, (▷ B α (sem_sig_eff_rec m A B) b) -∗ Φ b))%I.
 Proof. 
   etrans; [by apply sem_sig_eff_rec_unfold'|]. 
   by rewrite (iEff_tele_eq' [tele _ _] [tele _]) /=. 
 Qed.
 
-(* The sem_sig_eff_rec is monotonic. *)
+(* The sem_sig_eff_rec protocol is monotonic. *)
 Global Instance sem_sig_eff_rec_mono_prot {Σ} A B `{ NonExpansive2 A, NonExpansive2 B }:
-  MonoProt (@sem_sig_eff_rec Σ A B).
+  MonoProt (@sem_sig_eff_rec Σ OS A B).
 Proof.
   constructor. iIntros (???) "HΦ'".
-  rewrite !sem_sig_eff_rec_eq.
-  iIntros "(% & % & -> & Hτ & HκΦ)".
-  iExists α, v. iSplitR; first done. iFrame.
+  rewrite !sem_sig_eff_rec_eq /=.
+  iIntros "(% & % & <- & Hτ & HκΦ)".
+  iExists α, a. iSplitR; first done. iFrame. simpl.
   iIntros (b) "Hκ". iApply "HΦ'". by iApply "HκΦ".
 Qed.
 
-Lemma upcl_sem_sig_rec_eff {Σ} A B v Φ `{ NonExpansive2 A, NonExpansive2 B}:
-  iEff_car (upcl OS (sem_sig_eff_rec (Σ:=Σ) A B)) v Φ ⊣⊢
-    (∃ α a, ⌜ a = v ⌝ ∗ (▷ A α (sem_sig_eff_rec A B) a) ∗ 
-                        (∀ b, (▷ B α (sem_sig_eff_rec A B) b) -∗ Φ b))%I.
+(* The sem_sig_eff_rec protocol is persistently monotonic. *)
+Global Instance sem_sig_eff_rec_pers_mono_prot {Σ} A B `{ NonExpansive2 A, NonExpansive2 B }:
+  PersMonoProt (@sem_sig_eff_rec Σ MS A B).
+Proof.
+  constructor. iIntros (???) "#HΦ'".
+  rewrite !sem_sig_eff_rec_eq. simpl.
+  iIntros "(% & % & <- & Hτ & #HκΦ)".
+  iExists α, a. iSplitR; first done. iFrame. simpl.
+  iIntros "!# %b Hκ". iApply "HΦ'". by iApply "HκΦ".
+Qed.
+
+Lemma upcl_sem_sig_rec_eff {Σ} m A B v Φ `{ NonExpansive2 A, NonExpansive2 B}:
+  iEff_car (upcl m (sem_sig_eff_rec (Σ:=Σ) m A B)) v Φ ⊣⊢
+    (∃ α a, ⌜ select_m m a = v ⌝ ∗ (▷ A α (sem_sig_eff_rec m A B) a) ∗ 
+                        □? m (∀ b, (▷ B α (sem_sig_eff_rec m A B) b) -∗ Φ b))%I.
 Proof.
   assert (Hequiv:
-    iEff_car (upcl OS (sem_sig_eff_rec A B)) v Φ ≡ iEff_car (sem_sig_eff_rec A B) v Φ).
-  { f_equiv. apply non_dep_fun_equiv. by rewrite upcl_id. }
+    iEff_car (upcl m (sem_sig_eff_rec m A B)) v Φ ≡ iEff_car (sem_sig_eff_rec m A B) v Φ).
+  { f_equiv. apply non_dep_fun_equiv. destruct m; [by rewrite upcl_id|by rewrite pers_upcl_id]. }
   rewrite Hequiv. by apply sem_sig_eff_rec_eq.
 Qed.
 
 (* Notations. *)
+Notation "⟨⟩" := (sem_sig_nil, sem_sig_nil) : sem_sig_scope.
+Notation "⟨ ρ , ρ' ⟩" := (ρ%R, ρ'%R) : sem_sig_scope.
+Notation "⟨ ρ , ⟩" := (ρ%R, sem_sig_nil) : sem_sig_scope.
+Notation "⟨ , ρ' ⟩" := (sem_sig_nil, ρ'%R) : sem_sig_scope.
+Notation "'∀μTS:' θ , α , τ ⇒ κ" := (sem_sig_eff_rec OS (λ α θ, τ%T) (λ α θ, κ%T))
+  (at level 100, τ, κ at level 200) : sem_sig_scope.
+
+Notation "'∀μTSₘ:' θ , α , τ ⇒ κ" := (sem_sig_eff_rec MS (λ α θ, τ%T) (λ α θ, κ%T))
+  (at level 100, τ, κ at level 200) : sem_sig_scope.
+
+Notation "⊥" := sem_ty_void : sem_ty_scope.
 Notation "()" := sem_ty_unit : sem_ty_scope.
 Notation "'𝔹'" := (sem_ty_bool) : sem_ty_scope.
 Notation "'ℤ'" := (sem_ty_int) : sem_ty_scope.
@@ -290,10 +250,10 @@ Notation "'Ref' τ" := (sem_ty_ref τ%T)
 Notation "'Refᶜ' τ" := (sem_ty_ref_cpy τ%T) 
   (at level 50) : sem_ty_scope.
 
-Notation "'∀T:' α , { ρ } ,  C " := (sem_ty_forall ρ (λ α, C%T)) 
+Notation "'∀T:' α , ρs ,  C " := (sem_ty_forall ρs%R (λ α, C%T)) 
   (at level 180) : sem_ty_scope.
 
-Notation "'∀T:' α ,, C " := (sem_ty_forall sem_sig_nil (λ α, C%T)) 
+Notation "'∀T:' α ,, C " := (sem_ty_forall (sem_sig_nil, sem_sig_nil) (λ α, C%T)) 
   (at level 180) : sem_ty_scope.
 
 Notation "'∀S:' θ , C " := (sem_ty_sig_forall (λ θ, C%T)) 
@@ -305,29 +265,14 @@ Notation "'∃:' α , C " := (sem_ty_exists (λ α, C%T))
 Notation "'μT:' α , C " := (sem_ty_rec (λ α, C%T))
   (at level 180) : sem_ty_scope.
 
-Notation "⟨⟩" := sem_sig_nil : sem_sig_scope.
-Notation "'∀μTS:' θ , α , τ ⇒ κ" := (sem_sig_eff_rec (λ α θ, τ%T) (λ α θ, κ%T))
-  (at level 100, τ, κ at level 200) : sem_sig_scope.
-
-Notation "τ '-{' ρ ; Γ₁ ; Γ₂ '}-∘' κ" := (sem_ty_aarr Γ₁ Γ₂ ρ%R τ%T κ%T)
-  (at level 100, ρ, κ at level 200) : sem_ty_scope.
-Notation "τ '-{' ρ '}-∘' κ" := (sem_ty_aarr [] [] ρ%R τ%T κ%T)
-  (at level 100, ρ, κ at level 200) : sem_ty_scope.
-Notation "τ ⊸ κ" := (sem_ty_aarr [] [] sem_sig_nil τ%T κ%T)
+Notation "τ '-{' ρs '}-∘' κ" := (sem_ty_aarr ρs%R τ%T κ%T)
+  (at level 100, ρs, κ at level 200) : sem_ty_scope.
+Notation "τ ⊸ κ" := (sem_ty_aarr (sem_sig_nil, sem_sig_nil) τ%T κ%T)
   (at level 99, κ at level 200) : sem_ty_scope.
 
-Notation "τ '-{' ρ ; Γ₁ ; Γ₂ '}->' κ" := (sem_ty_uarr Γ₁ Γ₂ ρ%R τ%T κ%T)
-  (at level 100, ρ, κ at level 200) : sem_ty_scope.
-Notation "τ '-{' ρ '}->' κ" := (sem_ty_uarr [] [] ρ%R τ%T κ%T)
-  (at level 100, ρ, κ at level 200) : sem_ty_scope.
-Notation "τ → κ" := (sem_ty_uarr [] [] sem_sig_nil τ%T κ%T)
-  (at level 99, κ at level 200) : sem_ty_scope.
-
-Notation "τ '>-{' ρ ; Γ₁ ; Γ₂ '}-∘' κ" := (sem_ty_suarr Γ₁ Γ₂ ρ%R τ%T κ%T)
-  (at level 100, ρ, Γ₁, Γ₂, κ at level 200) : sem_ty_scope.
-Notation "τ '>-{' ρ '}-∘' κ" := (sem_ty_suarr [] [] ρ%R τ%T κ%T)
-  (at level 100, ρ, κ at level 200) : sem_ty_scope.
-Notation "τ >-∘ κ" := (sem_ty_suarr [] [] sem_sig_nil τ%T κ%T)
+Notation "τ '-{' ρs '}->' κ" := (sem_ty_uarr ρs%R τ%T κ%T)
+  (at level 100, ρs, κ at level 200) : sem_ty_scope.
+Notation "τ → κ" := (sem_ty_uarr (sem_sig_nil, sem_sig_nil) τ%T κ%T)
   (at level 99, κ at level 200) : sem_ty_scope.
 
 (* Derived Types *)
@@ -355,7 +300,7 @@ Section types_properties.
     repeat intros ?;
     unfold sem_ty_unit, sem_ty_int, sem_ty_bool, sem_ty_cpy,
            sem_ty_prod, sem_ty_sum, sem_ty_aarr,
-           sem_ty_uarr, sem_ty_suarr, sem_ty_ref, sem_ty_ref_cpy,
+           sem_ty_uarr, sem_ty_ref, sem_ty_ref_cpy,
            sem_ty_rec, sem_ty_list, sem_ty_forall, sem_ty_exists;
     repeat (f_equiv || done || intros ? || by apply non_dep_fun_dist).
 
@@ -368,20 +313,11 @@ Section types_properties.
   Global Instance sem_ty_sum_ne : NonExpansive2 (@sem_ty_sum Σ).
   Proof. solve_non_expansive. Qed.
 
-  Global Instance sem_ty_aarr_ne Γ₁ Γ₂: NonExpansive3 (sem_ty_aarr Γ₁ Γ₂).
+  Global Instance sem_ty_aarr_ne : NonExpansive3 sem_ty_aarr.
   Proof. solve_non_expansive. Qed.
 
-  Global Instance sem_ty_uarr_ne Γ₁ Γ₂ : NonExpansive3 (sem_ty_uarr Γ₁ Γ₂).
+  Global Instance sem_ty_uarr_ne : NonExpansive3 sem_ty_uarr.
   Proof. solve_non_expansive. Qed.
-
-  Global Instance sem_ty_suarr_ne Γ₁ Γ₂ : NonExpansive3 (sem_ty_suarr Γ₁ Γ₂).
-  Proof. 
-    intros ??????????. rewrite /sem_ty_suarr. 
-   apply fixpoint_ne.
-    intros ?. rewrite /sem_ty_suarr_pre. intros ?. 
-    repeat f_equiv; [by apply non_dep_fun_dist|done|].
-    intros ?. f_equiv. by apply non_dep_fun_dist.
-  Qed.
 
   Global Instance sem_ty_ref_ne : NonExpansive (@sem_ty_ref Σ _).
   Proof. solve_non_expansive. Qed.
@@ -389,8 +325,8 @@ Section types_properties.
   Global Instance sem_ty_ref_cpy_ne : NonExpansive (@sem_ty_ref_cpy Σ _).
   Proof. solve_non_expansive. Qed.
 
-  Global Instance sem_ty_forall_ne n ρ :
-    Proper (pointwise_relation _ (dist n) ==> dist n) (sem_ty_forall ρ).
+  Global Instance sem_ty_forall_ne n ρs :
+    Proper (pointwise_relation _ (dist n) ==> dist n) (sem_ty_forall ρs).
   Proof. intros ????. unfold sem_ty_forall; repeat f_equiv. Qed.
 
   Global Instance sem_ty_exist_ne n :
@@ -429,18 +365,11 @@ Section types_properties.
   Global Instance sem_ty_sum_proper : Proper ((≡) ==> (≡) ==> (≡)) (@sem_ty_sum Σ).
   Proof. solve_non_expansive. Qed.
 
-  Global Instance sem_ty_aarr_proper Γ₁ Γ₂ : Proper ((≡) ==> (≡) ==> (≡) ==> (≡)) (sem_ty_aarr Γ₁ Γ₂).
+  Global Instance sem_ty_aarr_proper : Proper ((≡) ==> (≡) ==> (≡) ==> (≡)) sem_ty_aarr.
   Proof. solve_non_expansive. Qed.
 
-  Global Instance sem_ty_uarr_proper Γ₁ Γ₂ : Proper ((≡) ==> (≡) ==> (≡) ==> (≡)) (sem_ty_uarr Γ₁ Γ₂).
+  Global Instance sem_ty_uarr_proper : Proper ((≡) ==> (≡) ==> (≡) ==> (≡)) sem_ty_uarr.
   Proof. solve_non_expansive. Qed.
-
-  Global Instance sem_ty_suarr_proper Γ₁ Γ₂ : Proper ((≡) ==> (≡) ==> (≡) ==> (≡)) (sem_ty_suarr Γ₁ Γ₂).
-  Proof. 
-    intros ?????????. apply equiv_dist=>n.
-    apply sem_ty_suarr_ne=> A; [by apply equiv_dist| |];
-    apply non_dep_fun_dist; by apply equiv_dist. 
-  Qed.
 
   Global Instance sem_ty_ref_proper : Proper ((≡) ==> (≡)) (@sem_ty_ref Σ _).
   Proof. intros ????. unfold sem_ty_ref; by repeat f_equiv. Qed.
@@ -448,8 +377,8 @@ Section types_properties.
   Global Instance sem_ty_ref_cpy_proper : Proper ((≡) ==> (≡)) (@sem_ty_ref_cpy Σ _).
   Proof. intros ????. unfold sem_ty_ref_cpy; by repeat f_equiv. Qed.
 
-  Global Instance sem_ty_forall_proper ρ:
-    Proper (pointwise_relation _ (≡) ==> (≡)) (sem_ty_forall ρ).
+  Global Instance sem_ty_forall_proper ρs :
+    Proper (pointwise_relation _ (≡) ==> (≡)) (sem_ty_forall ρs).
   Proof. intros ????; unfold sem_ty_forall; repeat f_equiv. Qed.
 
   Global Instance sem_ty_exist_proper :
