theories/logic/compatibility.v
@@ -27,7 +27,6 @@ From affine_tes.logic Require Import sem_types.
 From affine_tes.logic Require Import sem_env.
 From affine_tes.logic Require Import sem_sub_typing.
 From affine_tes.logic Require Import sem_operators.
-From affine_tes.logic Require Import reasoning.
 
 
 Open Scope bi_scope.
@@ -43,8 +42,8 @@ Section compatibility.
   Lemma sem_typed_val Γ τ v : 
     ⊨ᵥ v : τ -∗ Γ ⊨ v : ⟨⟩ : τ ⊨ Γ.
   Proof.
-    iIntros "#Hv !# %Φ %vs HΓ HΦ /=".
-    iApply ewp_value. iApply "HΦ". iIntros "{$Hv} {$HΓ}".
+    iIntros "#Hv !# %vs HΓ /=".
+    iApply ewp_value. iIntros "{$Hv} {$HΓ}".
   Qed.
 
   (* Base rules *)
@@ -52,63 +51,68 @@ Section compatibility.
   Lemma sem_typed_unit Γ : 
     ⊢ Γ ⊨ #() : ⟨⟩ : () ⊨ Γ.
   Proof.
-    iIntros (Φ vs) "!# HΓ₁ HΦ //=". iApply ewp_value. 
-    iApply "HΦ". by iFrame.
+    iIntros (vs) "!# HΓ₁ //=". iApply ewp_value. by iFrame.
   Qed.
   
   Lemma sem_typed_bool Γ (b : bool) : 
     ⊢ Γ ⊨ #b : ⟨⟩ : 𝔹 ⊨ Γ.
   Proof.
-    iIntros (Φ vs) "!# HΓ₁ HΦ //=". iApply ewp_value. 
-    iApply "HΦ". iSplitR; first (iExists b); done.
+    iIntros (vs) "!# HΓ₁ //=". iApply ewp_value. 
+    iSplitR; first (iExists b); done.
   Qed.
   
   Lemma sem_typed_int Γ (i : Z) : 
     ⊢ Γ ⊨ #i : ⟨⟩ : ℤ ⊨ Γ.
   Proof.
-    iIntros (Φ vs) "!# HΓ₁ HΦ //=". iApply ewp_value. 
-    iApply "HΦ". iSplitR; first (iExists i); done.
+    iIntros (vs) "!# HΓ₁ //=". iApply ewp_value. 
+    iSplitR; first (iExists i); done.
   Qed.
   
   Lemma sem_typed_var Γ x τ : 
     ⊢ (x, τ) :: Γ ⊨ x : ⟨⟩ : τ ⊨ Γ.
   Proof.
-    iIntros (Φ vs) "!# /= [%v (%Hrw & Hτ & HΓ₁)] HΦ /=". 
-    rewrite Hrw. iApply ewp_value. iApply "HΦ". iFrame.
+    iIntros (vs) "!# /= [%v (%Hrw & Hτ & HΓ₁)] /=". 
+    rewrite Hrw. iApply ewp_value. iFrame.
   Qed.
 
-  Lemma sem_typed_closure f x e τ ρ κ :
+  Lemma sem_typed_bot_in_env Γ₁ Γ₂ e x τ : 
+    ⊢ (x, @sem_ty_void Σ) :: Γ₁ ⊨ e : ⟨⟩ : τ ⊨ Γ₂.
+  Proof.
+    iIntros (vs) "!# /= [%v (%Hrw & [] & _)] /=". 
+  Qed.
+
+  Lemma sem_typed_closure f x e τ ρs κ :
     match f with BNamed f => BNamed f ≠ x | BAnon => True end →
-    (x, τ) ::? (f, τ -{ ρ }-> κ) ::? [] ⊨ e : ρ : κ ⊨ [] -∗ 
-    ⊨ᵥ (rec: f x := e) : (τ -{ ρ }-> κ).
+    (x, τ) ::? (f, τ -{ ρs }-> κ) ::? [] ⊨ e : ρs : κ ⊨ [] -∗ 
+    ⊨ᵥ (rec: f x := e) : (τ -{ ρs }-> κ).
   Proof.
       iIntros (?) "#He !#". iLöb as "IH".
-      iIntros "%v !# %ws _ Hτ /=". 
-      rewrite env_dom_nil env_sem_typed_empty /=.
+      iIntros "%v !# Hτ /=". 
       ewp_pure_steps. destruct x as [|x]; destruct f as [|f]; simpl.
       - rewrite - {3} [e]subst_map_empty. 
-        iApply "He"; first done.
-        iIntros (w) "[$ _]".
+        iApply (ewp_pers_mono with "[He]"); first (by iApply "He").
+        iIntros "!# % [$ _] //=". 
       - rewrite -subst_map_singleton.
-        iApply ("He" with "[Hτ] []"); first solve_env.
-        iIntros (w) "[$ _]".
+        iApply ewp_pers_mono; [iApply "He"; solve_env|solve_env].
+        iIntros "!# % [$ _] //=".
       - rewrite -subst_map_singleton.
-        iApply ("He" with "[Hτ] []"); first solve_env.
-        iIntros (w) "[$ _]".
+        iApply (ewp_pers_mono with "[Hτ]"); [iApply "He"; solve_env|solve_env].
+        iIntros "!# % [$ _] //=".
       - rewrite -(subst_map_singleton f) -subst_map_singleton subst_map_union.
-        iApply ("He" with "[Hτ]"); [|iIntros (?) "[$ _]"].
+        iApply (ewp_pers_mono with "[Hτ]"); [iApply "He"|iIntros "!# % [$ _] //="].
         rewrite -insert_union_singleton_r; [solve_env|apply lookup_singleton_ne];
         intros ?; simplify_eq.
   Qed.
 
-  Lemma sem_typed_Tclosure e τ ρ :
-    (∀ α, ⊨ e : ρ : τ α) -∗ 
-    ⊨ᵥ (Λ: e) : (∀T: α, { ρ }, τ α).
+  Lemma sem_typed_Tclosure e τ ρs :
+    (∀ α, ⊨ e : ρs : τ α) -∗ 
+    ⊨ᵥ (Λ: e) : (∀T: α, ρs , τ α).
   Proof.
     iIntros "#He !# %u !#". ewp_pure_steps.
     rewrite - {2} [e]subst_map_empty.
-    iSpecialize ("He" $! u (τ u) ∅).
-    iApply "He"; first done. iIntros (?) "[$ _]".
+    iSpecialize ("He" $! u).
+    iApply (ewp_pers_mono with "[He]"); [iApply "He"|]; first done. 
+    iIntros "!# % [$ _] //=".
   Qed.
 
   (* Signature abstraction and application *)
@@ -118,91 +122,89 @@ Section compatibility.
   Proof.
     iIntros "#He !# %ρ /=".
     ewp_pure_steps. rewrite - {2} [e]subst_map_empty. 
-    iApply (ewp_mono with "[He]").
-    { iApply "He"; [done|iIntros (?) "[H _]"; iApply "H"].  }
-    iIntros (v) "$ //".
+    iApply (ewp_pers_mono with "[He]"); [by iApply "He"|].
+    iIntros "!# % [$ _] //=". 
   Qed.
 
-  Lemma sem_typed_closure_to_unrestricted x e τ ρ κ Γ₁ Γ₂ :
-    ⊨ᵥ (λ*λ: env_dom Γ₁, x, e) : (τ -{ ρ ; Γ₁ ; Γ₂ }-∘ κ) -∗
-    ⊨ᵥ (λ*λ: env_dom Γ₁, x, e) : (τ -{ ρ ; Γ₁ ; Γ₂ }-> κ).
+  Lemma sem_typed_closure_to_unrestricted x e τ ρs κ :
+    ⊨ᵥ (λ: x, e) : (τ -{ ρs }-∘ κ) -∗
+    ⊨ᵥ (λ: x, e) : (τ -{ ρs }-> κ).
   Proof. 
-    iIntros "#He !# %w !# %vs HΓ₁ Hτ". 
-    iSpecialize ("He" $! w vs).
-    iApply ("He" with "HΓ₁ Hτ").
+    iIntros "#He !# %w !# Hτ". 
+    iSpecialize ("He" $! w).
+    iApply ("He" with "Hτ").
   Qed.
 
   (* Subsumption rule *)
   
-  Lemma sem_typed_sub Γ₁ Γ₁' Γ₂ Γ₂' e ρ ρ' τ τ':
+  Lemma sem_typed_sub Γ₁ Γ₁' Γ₂ Γ₂' e ρs ρs' τ τ':
     Γ₁  ≤E Γ₁' →
     Γ₂' ≤E Γ₂ →
-    ρ'  ≤R ρ → 
+    ρs' ≤Rs ρs → 
     τ'  ≤T τ →
-    Γ₁' ⊨ e : ρ' : τ' ⊨ Γ₂' -∗ Γ₁ ⊨ e : ρ : τ ⊨ Γ₂.
+    Γ₁' ⊨ e : ρs' : τ' ⊨ Γ₂' -∗ Γ₁ ⊨ e : ρs : τ ⊨ Γ₂.
   Proof.
-    iIntros (HΓ₁le HΓ₂le Hρle Hτle) "#He !# %Φ %vs HΓ₁ HΦ //=".
+    iIntros (HΓ₁le HΓ₂le [Hρle₁ Hρle₂] Hτle) "#He !# %vs HΓ₁ //=".
     rewrite HΓ₁le.
-    iApply ewp_os_prot_mono.
-    { iApply Hρle. }
-    iApply ("He" with "HΓ₁").
-    iIntros (v) "[Hτ' HΓ₂]". iApply "HΦ".
-    rewrite HΓ₂le. iFrame.
-    by iApply Hτle.
+    iApply ewp_os_prot_mono; [iApply Hρle₁|].
+    iApply ewp_ms_prot_mono; [iApply Hρle₂|].
+    iApply (ewp_pers_mono with "[HΓ₁]"); first (by iApply "He").
+    iIntros "!# % [Hτ HΓ₂] //=".
+    rewrite HΓ₂le Hτle. by iFrame.
   Qed. 
   
   (* Convenient Subsumption rules *)
-  Lemma sem_typed_sub_ty τ' τ Γ₁ Γ₂ e ρ :
+  Lemma sem_typed_sub_ty τ' τ Γ₁ Γ₂ e ρs :
   τ' ≤T τ →
-  (Γ₁ ⊨ e : ρ : τ' ⊨ Γ₂) -∗ Γ₁ ⊨ e : ρ : τ ⊨ Γ₂.
+  (Γ₁ ⊨ e : ρs : τ' ⊨ Γ₂) -∗ Γ₁ ⊨ e : ρs : τ ⊨ Γ₂.
   Proof.
     iIntros (Hτ).
-    iApply (sem_typed_sub Γ₁ Γ₁ Γ₂ Γ₂ _ ρ ρ);
-      (apply sig_le_refl || apply env_le_refl || done). 
+    iApply (sem_typed_sub Γ₁ Γ₁ Γ₂ Γ₂ _ ρs ρs);
+      (apply sigs_le_refl || apply env_le_refl || done). 
   Qed.
 
-  Lemma sem_typed_sub_sig ρ ρ' Γ₁ Γ₂ e τ :
-    ρ' ≤R ρ →
-    (Γ₁ ⊨ e : ρ' : τ ⊨ Γ₂) -∗ Γ₁ ⊨ e : ρ : τ ⊨ Γ₂.
+  Lemma sem_typed_sub_sig ρs ρs' Γ₁ Γ₂ e τ :
+    ρs' ≤Rs ρs →
+    (Γ₁ ⊨ e : ρs' : τ ⊨ Γ₂) -∗ Γ₁ ⊨ e : ρs : τ ⊨ Γ₂.
   Proof.
     iIntros (Hρ).
-    iApply (sem_typed_sub Γ₁ Γ₁ Γ₂ Γ₂ _ ρ ρ' τ τ);
-      (apply sig_le_refl || apply env_le_refl || apply ty_le_refl || done).
+    iApply (sem_typed_sub Γ₁ Γ₁ Γ₂ Γ₂ _ ρs ρs' τ τ);
+      (apply sigs_le_refl || apply env_le_refl || apply ty_le_refl || done).
   Qed.
 
-  Lemma sem_typed_sub_nil Γ₁ Γ₂ e τ ρ :
-    (Γ₁ ⊨ e : ⟨⟩ : τ ⊨ Γ₂) -∗ Γ₁ ⊨ e : ρ : τ ⊨ Γ₂.
-  Proof. iApply sem_typed_sub_sig. apply sig_le_nil. Qed.
+  Lemma sem_typed_sub_nil Γ₁ Γ₂ e τ ρs :
+    (Γ₁ ⊨ e : ⟨⟩ : τ ⊨ Γ₂) -∗ Γ₁ ⊨ e : ρs : τ ⊨ Γ₂.
+  Proof. iApply sem_typed_sub_sig. apply sigs_le_nil. Qed.
   
-  Lemma sem_typed_sub_env Γ₁ Γ₁' Γ₂ e ρ τ :
+  Lemma sem_typed_sub_env Γ₁ Γ₁' Γ₂ e ρs τ :
     Γ₁ ≤E Γ₁' →
-    (Γ₁' ⊨ e : ρ : τ ⊨ Γ₂) -∗ Γ₁ ⊨ e : ρ : τ ⊨ Γ₂.
+    (Γ₁' ⊨ e : ρs : τ ⊨ Γ₂) -∗ Γ₁ ⊨ e : ρs : τ ⊨ Γ₂.
   Proof.
     iIntros (HΓ₁).
-    iApply (sem_typed_sub Γ₁ Γ₁' Γ₂ Γ₂ _ ρ ρ τ τ);
-      (apply sig_le_refl || apply env_le_refl || apply ty_le_refl || done).
+    iApply (sem_typed_sub Γ₁ Γ₁' Γ₂ Γ₂ _ ρs ρs τ τ);
+      (apply sigs_le_refl || apply env_le_refl || apply ty_le_refl || done).
   Qed.
 
-  Lemma sem_typed_swap_second Γ₁ Γ₂ x y e ρ τ₁ τ₂ κ :
-    ((y, τ₂) :: (x, τ₁) :: Γ₁ ⊨ e : ρ : κ ⊨ Γ₂) -∗ 
-    ((x, τ₁) :: (y, τ₂) :: Γ₁ ⊨ e : ρ : κ ⊨ Γ₂).
+  Lemma sem_typed_swap_second Γ₁ Γ₂ x y e ρs τ₁ τ₂ κ :
+    ((y, τ₂) :: (x, τ₁) :: Γ₁ ⊨ e : ρs : κ ⊨ Γ₂) -∗ 
+    ((x, τ₁) :: (y, τ₂) :: Γ₁ ⊨ e : ρs : κ ⊨ Γ₂).
   Proof.
     iIntros "He".
     iApply sem_typed_sub_env; [apply env_le_swap_second|iApply "He"].
   Qed.
 
-  Lemma sem_typed_swap_third Γ₁ Γ₂ x y z e ρ τ₁ τ₂ τ₃ κ :
-    ((z, τ₃) :: (x, τ₁) :: (y, τ₂) :: Γ₁ ⊨ e : ρ : κ ⊨ Γ₂) -∗ 
-    ((x, τ₁) :: (y, τ₂) :: (z, τ₃) :: Γ₁ ⊨ e : ρ : κ ⊨ Γ₂).
+  Lemma sem_typed_swap_third Γ₁ Γ₂ x y z e ρs τ₁ τ₂ τ₃ κ :
+    ((z, τ₃) :: (x, τ₁) :: (y, τ₂) :: Γ₁ ⊨ e : ρs : κ ⊨ Γ₂) -∗ 
+    ((x, τ₁) :: (y, τ₂) :: (z, τ₃) :: Γ₁ ⊨ e : ρs : κ ⊨ Γ₂).
   Proof.
     iIntros "He".
     iApply sem_typed_sub_env; [|iApply "He"].
     eapply env_le_trans; apply env_le_swap_third.
   Qed.
 
-  Lemma sem_typed_swap_fourth Γ₁ Γ₂ x y z z' e ρ τ₁ τ₂ τ₃ τ₄ κ :
-    ((z', τ₄) :: (x, τ₁) :: (y, τ₂) :: (z, τ₃) :: Γ₁ ⊨ e : ρ : κ ⊨ Γ₂) -∗ 
-    ((x, τ₁) :: (y, τ₂) :: (z, τ₃) :: (z', τ₄) :: Γ₁ ⊨ e : ρ : κ ⊨ Γ₂).
+  Lemma sem_typed_swap_fourth Γ₁ Γ₂ x y z z' e ρs τ₁ τ₂ τ₃ τ₄ κ :
+    ((z', τ₄) :: (x, τ₁) :: (y, τ₂) :: (z, τ₃) :: Γ₁ ⊨ e : ρs : κ ⊨ Γ₂) -∗ 
+    ((x, τ₁) :: (y, τ₂) :: (z, τ₃) :: (z', τ₄) :: Γ₁ ⊨ e : ρs : κ ⊨ Γ₂).
   Proof.
     iIntros "He".
     iApply sem_typed_sub_env; [|iApply "He"].
@@ -210,581 +212,341 @@ Section compatibility.
     apply env_le_swap_fourth.
   Qed.
 
-  Lemma sem_typed_contraction Γ₁ Γ₂ x e ρ τ κ :
+  Lemma sem_typed_swap_env_singl Γ₁ Γ₂ x e ρs τ κ :
+    (Γ₁ ++ [(x, τ)] ⊨ e : ρs : κ ⊨ Γ₂) -∗ 
+    ((x, τ) :: Γ₁ ⊨ e : ρs : κ ⊨ Γ₂). 
+  Proof.
+    iIntros "He".
+    iApply sem_typed_sub_env; [|iApply "He"].
+    apply env_le_swap_env_singl.
+  Qed.
+
+  Lemma sem_typed_contraction Γ₁ Γ₂ x e ρs τ κ :
     copy_ty τ →
-    (x, τ) :: (x, τ) :: Γ₁ ⊨ e : ρ : κ ⊨ Γ₂ -∗ 
-    (x, τ) :: Γ₁ ⊨ e : ρ : κ ⊨ Γ₂.
+    (x, τ) :: (x, τ) :: Γ₁ ⊨ e : ρs : κ ⊨ Γ₂ -∗ 
+    (x, τ) :: Γ₁ ⊨ e : ρs : κ ⊨ Γ₂.
   Proof.
     iIntros (?) "He".
     iApply sem_typed_sub_env; 
       [by apply env_le_copy_contraction|iApply "He"].
   Qed.
 
-  Lemma sem_typed_weaken Γ₁ Γ₂ x e ρ τ κ :
-    (Γ₁ ⊨ e : ρ : κ ⊨ Γ₂) -∗ ((x, τ) :: Γ₁ ⊨ e : ρ : κ ⊨ Γ₂).
+  Lemma sem_typed_weaken Γ₁ Γ₂ x e ρs τ κ :
+    (Γ₁ ⊨ e : ρs : κ ⊨ Γ₂) -∗ ((x, τ) :: Γ₁ ⊨ e : ρs : κ ⊨ Γ₂).
   Proof.
     iIntros "He".
     iApply sem_typed_sub_env; [apply env_le_weaken|iApply "He"].
   Qed.
 
-  Lemma sem_typed_frame Γ₁ e ρ x τ κ Γ₂:
-    Γ₁ ⊨ e : ρ : κ ⊨ Γ₂ -∗
-    (x, τ) :: Γ₁ ⊨ e : ρ : κ ⊨ (x, τ) :: Γ₂.
+  Lemma sem_typed_frame_os Γ₁ e ρ x τ κ Γ₂:
+    Γ₁ ⊨ e : ⟨ ρ, ⟩ : κ ⊨ Γ₂ -∗
+    (x, τ) :: Γ₁ ⊨ e : ⟨ ρ, ⟩ : κ ⊨ (x, τ) :: Γ₂.
   Proof.
-    iIntros "#He %Φ %vs !# (%v & %Hrw & Hτ & HΓ₁) HΦ".
-    iApply ("He" with "HΓ₁"). iIntros (w) "[Hκ HΓ₂]".
-    iApply "HΦ". solve_env.
+    iIntros "#He %vs !# (%v & %Hrw & Hτ & HΓ₁)".
+    iApply (ewp_mono with "[HΓ₁]"); first (by iApply "He").
+    iIntros (w) "[Hκ HΓ₂]". solve_env.
+  Qed.
+
+  Lemma sem_typed_frame_env_os Γ₁ Γ' e ρ τ Γ₂ :
+    Γ₁ ⊨ e : ⟨ ρ, ⟩ : τ ⊨ Γ₂ -∗
+    Γ' ++ Γ₁ ⊨ e : ⟨ ρ, ⟩ : τ ⊨ Γ' ++ Γ₂.
+  Proof.
+    iIntros "#He %vs !# HΓ'Γ₁".
+    iDestruct (env_sem_typed_app with "HΓ'Γ₁") as "[HΓ' HΓ₁]".
+    iInduction Γ' as [|[x κ]] "IH".
+    { simpl. by iApply "He". }
+    iDestruct "HΓ'" as "(%v & %Hrw & Hκ & HΓ'')".
+    iApply (ewp_mono with "[HΓ'' HΓ₁]").
+    { iApply ("IH" with "HΓ'' HΓ₁"). }
+    iIntros (w) "[$ HΓ] !>". solve_env.
+  Qed.
+
+  Lemma sem_typed_frame_ms Γ₁ e ρs x τ κ Γ₂:
+    copy_ty τ →
+    Γ₁ ⊨ e : ρs : κ ⊨ Γ₂ -∗
+    (x, τ) :: Γ₁ ⊨ e : ρs : κ ⊨ (x, τ) :: Γ₂.
+  Proof.
+    iIntros (Hcpy) "#He %vs !# (%v & %Hrw & Hτ & HΓ₁)".
+    rewrite Hcpy. iDestruct "Hτ" as "#Hτ".
+    iApply (ewp_pers_mono with "[HΓ₁]"); first (by iApply "He").
+    iIntros "!# % [Hκ HΓ₂]". solve_env.
   Qed.
 
   (* λ-calculus rules *)
 
-  Lemma sem_typed_afun_mult Γ₁ Γ₂ Δ₁ Δ₂ x e τ ρ κ: 
-    x ∉ (env_dom Γ₁) → x ∉ (env_dom Δ₁) → x ∉ (env_dom Γ₂) →
-    env_dom Δ₂ ⊆ env_dom Δ₁ →
-    env_dom Γ₁ ## env_dom Δ₁ →
-    (x,τ) ::? Δ₁ ++ Γ₁ ⊨ e : ρ : κ ⊨ Δ₂ -∗
-    Γ₁ ++ Γ₂ ⊨ (λ*λ: env_dom Δ₁, x, e) : ⟨⟩ : (τ -{ ρ ; Δ₁ ; Δ₂ }-∘ κ) ⊨ Γ₂.
-  Proof.
-    iIntros (?????) "#He !# %Φ %vs HΓ₁₂ HΦ //=".
-    iDestruct (env_sem_typed_app with "HΓ₁₂") as "[HΓ₁ HΓ₂]".
-    rewrite subst_map_ctx_lambda /=. 
-    destruct Δ₁ as [|[z ι] Δ₁'].
-    - rewrite env_dom_nil delete_list_nil. simpl. 
-      replace Δ₂ with ([] : env Σ) 
-          by (symmetry; apply (map_eq_nil fst); by apply list_nil_subseteq). 
-      ewp_pure_steps. iApply "HΦ". iFrame.
-      iIntros (w ws) "_ Hτ". rewrite env_dom_nil /=.
-      ewp_pure_steps. rewrite subst'_subst_map_insert.
-      iApply ("He" with "[Hτ HΓ₁] []").
-      { destruct x; solve_env. }
-      iIntros (u) "[$ _]".
-    - rewrite env_dom_cons delete_list_cons. iSimpl.
-      ewp_pure_steps. iApply "HΦ". iFrame.
-      iIntros (u ws) "HΔ₁ Hτ". 
-      set Δ₁ := (z, ι) :: Δ₁'.
-      set e' := subst_map _ e.
-      iApply (ewp_bind [AppLCtx _]); first done.
-      ewp_bottom.
-      iApply (ewp_app_mult with "[HΔ₁]"); first done. iIntros "HΔ₁".
-      simpl. ewp_pure_steps.
-      rewrite /e' env_dom_cons subst_map_union -binder_delete_union subst'_subst_map_insert -(env_dom_cons _ ι).
-      iApply ("He" with "[HΔ₁ Hτ HΓ₁]"); destruct x as [|x]. 
-      + rewrite app_comm_cons env_sem_typed_app -/Δ₁. iSimpl.
-        iSplitL "HΔ₁".
-        { rewrite (env_sem_typed_difference_delete Δ₁); last reflexivity. 
-          by rewrite (env_sem_typed_delete_union Δ₁); last reflexivity. }
-        { rewrite (env_sem_typed_delete_disjoint Γ₁ Δ₁); last done. 
-        by iApply env_sem_typed_union. }
-      + iExists u. iSplitL ""; first (iPureIntro; apply lookup_insert). iFrame.
-        rewrite app_comm_cons -/Δ₁.
-        rewrite -(env_sem_typed_insert (Δ₁ ++ Γ₁) _ x u);
-          last (rewrite env_dom_app; by eapply not_elem_of_app).
-        rewrite env_sem_typed_app.
-        rewrite (env_sem_typed_difference_delete Δ₁); last reflexivity.
-        rewrite (env_sem_typed_delete_union Δ₁); last reflexivity. iFrame.
-        rewrite (env_sem_typed_delete_disjoint Γ₁ Δ₁); last done. 
-        by iApply (env_sem_typed_union Γ₁). 
-      + iIntros (w) "[$ HΔ₂Γ₁] /=". 
-        rewrite -(env_sem_typed_delete_union Δ₂ Δ₁); last done. 
-        by rewrite -(env_sem_typed_difference_delete Δ₂ Δ₁).
-      + iIntros (w) "[$ HΔ₂Γ₁] /=". 
-        assert (x ∉ env_dom Δ₂).
-        { intros ?. apply H0. 
-          destruct (elem_of_subseteq (env_dom Δ₂) (env_dom Δ₁)) as [H' _]. 
-          by apply H'. }
-        rewrite -env_sem_typed_insert; last done.
-        rewrite -(env_sem_typed_delete_union Δ₂ Δ₁); last done. 
-        rewrite -(env_sem_typed_difference_delete Δ₂ Δ₁); last done. iFrame. 
-  Qed.
-
-  Lemma sem_typed_afun Γ₁ Γ₂ x e τ ρ κ: 
+  Lemma sem_typed_afun Γ₁ Γ₂ x e τ ρs κ: 
     x ∉ (env_dom Γ₁) → x ∉ (env_dom Γ₂) →
-    (x,τ) ::? Γ₁ ⊨ e : ρ : κ ⊨ [] -∗
-    Γ₁ ++ Γ₂ ⊨ (λ: x, e) : ⟨⟩ : (τ -{ ρ }-∘ κ) ⊨ Γ₂.
+    (x,τ) ::? Γ₁ ⊨ e : ρs : κ ⊨ [] -∗
+    Γ₁ ++ Γ₂ ⊨ (λ: x, e) : ⟨⟩ : (τ -{ ρs }-∘ κ) ⊨ Γ₂.
   Proof.
-    intros ??.
-    rewrite [(λ: x, _)%E](@ctx_lambda_env_dom_nil Σ).
-    iApply (sem_typed_afun_mult _ _ [] []); solve_sidecond.
-  Qed.
-
-  Lemma sem_typed_lambdas_norm Γ Γ' Δ₁ Δ₂ f x ρ e τ κ :
-    env_dom Δ₂ ⊆ env_dom Δ₁ →
-    x ∉ env_dom Δ₁ → f ∉ env_dom Δ₁ → f ≠ x →
-    Γ ⊨ e : ρ : (τ -{ ρ }-> (() -{ ρ ; Δ₁; Δ₂ }-∘ κ)) ⊨ Γ' -∗
-    Γ ⊨ (lambdas_norm f x (env_dom Δ₁) e) : ρ : (τ -{ ρ ; Δ₁; Δ₂ }-> κ) ⊨ Γ'.
-  Proof.
-    iIntros (Hdis Hx Hf Hfx) "#He %Φ %vs !# HΓ HΦ". 
-    rewrite /lambdas_norm /=. 
-    iApply (ewp_bind [AppRCtx _]); first done.
-    iApply ("He" with "HΓ"). iIntros (w) "[#Hτuκ HΓ'] /=".
-    ewp_pure_steps. 
-    rewrite -subst_map_singleton subst_map_ctx_lambda delete_list_singleton_ne; last done.
-    rewrite /= subst_map_app_mult /= lookup_delete lookup_delete_ne; last done.
-    rewrite lookup_insert. 
-    replace (map (subst_map (delete x {[f := w]})) (map Var (env_dom Δ₁))) with
-            (map Var (env_dom Δ₁)).
-    2: { clear - Δ₁ x f w Hx Hf Hfx. 
-         induction Δ₁ as [|[z ι] Δ₁']; first done. rewrite env_dom_cons /=.
-         rewrite env_dom_cons in Hx Hf.
-         edestruct (not_elem_of_cons (env_dom Δ₁') x)  as [[] _]; first done.
-         edestruct (not_elem_of_cons (env_dom Δ₁') f)  as [[] _]; first done.
-         rewrite lookup_delete_ne; last done. rewrite lookup_singleton_ne; last done.
-         by rewrite -IHΔ₁'. }
-    destruct Δ₁ as [|[z ι] Δ₁'] eqn:HΔ₁eq.
-    - rewrite env_dom_nil /=. ewp_pure_steps.
-      iApply "HΦ". iIntros "{$HΓ'} %u %us !# _ Hτ /=".
-      rewrite env_dom_nil /=. ewp_pure_steps. rewrite decide_True; last done.
-      iApply (ewp_bind [AppLCtx _]); first done.
-      iApply (ewp_mono with "[Hτuκ Hτ]"); [by iApply "Hτuκ"|].
-      iIntros (?) "[Hu _] !> /=". by iApply "Hu".
-      Unshelve. apply empty.
-    - rewrite {1}env_dom_cons env_dom_nil /=. ewp_pure_steps. iApply "HΦ".
-      iIntros "{$HΓ'} %u %us !# HΔ₁ Hτ". iApply (ewp_bind [AppLCtx _]); first done.
-      iApply (ewp_app_mult with "HΔ₁"). iIntros "HΔ₁".
-      simpl. ewp_pure_steps. rewrite -subst_map_insert subst_map_app_mult /=.
-      rewrite lookup_insert map_map_subst_map -HΔ₁eq. 
-      rewrite -HΔ₁eq in Hx Hf Hdis.
-      set uus := (<[x:=u]> (us ∖ delete (env_dom Δ₁) us)).
-      iDestruct (subst_map_var Δ₁ uus with "[HΔ₁]") as "[%uus' %Hrwuus']".
-      { rewrite -env_sem_typed_insert; last done.
-        by rewrite env_sem_typed_difference_delete. }
-      rewrite Hrwuus' app_mult_cons. 
-      replace ([ #() : expr ]) with (map Val [ #() : val ]) by done.
-      rewrite -map_app. iApply ewp_bind_app_mult.
-      iApply (ewp_mono with "[Hτuκ Hτ] [HΔ₁]"); [by iApply "Hτuκ"|].
-      iIntros (q) "[Hq _] !> /=". rewrite map_app /= -app_mult_cons -Hrwuus'.
-      iSpecialize ("Hq" $! #() uus with "[HΔ₁] []"); try done.
-      { rewrite -env_sem_typed_insert; last done.
-        by rewrite env_sem_typed_difference_delete. }
-      iApply (ewp_mono with "Hq").
-      assert (x ∉ env_dom Δ₂).
-      { intros ?. apply Hx. by eapply (elem_of_subseteq (env_dom Δ₂)); done. }
-      iIntros (?) "[$ HΔ₁] !>". rewrite /uus.
-      { rewrite -env_sem_typed_insert; last done. 
-        by rewrite -env_sem_typed_difference_delete. }
-      Unshelve. apply empty.
-  Qed.
-
-  Lemma sem_typed_ufun_mult Γ₁ Γ₂ Δ₁ Δ₂ f x e τ ρ κ:
-    x ∉ (env_dom Γ₁) → f ∉ (env_dom Γ₁) → f ∉ (env_dom Δ₁) → x ∉ (env_dom Δ₁) →
-    env_dom Δ₂ ⊆ env_dom Δ₁ →
-    env_dom Γ₁ ## env_dom Δ₁ →
-    x ≠ f →
-    copy_env Γ₁ →
-    (x, τ) :: (f, τ -{ ρ ; Δ₁ ; Δ₂ }-> κ) :: Δ₁ ++ Γ₁ ⊨ e : ρ : κ ⊨ Δ₂ -∗
-    Γ₁ ++ Γ₂ ⊨ (rec*: f , env_dom Δ₁, x,  e) : ρ : (τ -{ ρ ; Δ₁ ; Δ₂ }-> κ) ⊨ Γ₂.
-  Proof.
-    iIntros (??????? HcpyΓ₁) "#He !# %Φ %vs HΓ₁₂ HΦ".
+    iIntros (??) "#He !# %vs HΓ₁₂ //=".
     iDestruct (env_sem_typed_app with "HΓ₁₂") as "[HΓ₁ HΓ₂]".
-    iApply (ewp_mono _ _ (λ v, (τ -{ ρ; Δ₁; Δ₂ }-> κ) v ∗ ⟦ Γ₂ ⟧ vs) with "[HΓ₁ HΓ₂] [HΦ]");
-      last (iIntros (?) "[Hτκ HΓ₂] !>"; iApply "HΦ"; iFrame). 
-    iApply (ewp_frame_r with "[HΓ₁] HΓ₂").
-    iApply (sem_typed_lambdas_norm Γ₁ [] Δ₁ Δ₂ f x ρ _ τ κ with "[] HΓ₁"); 
-      try done; last (iIntros (?) "[$ _] $! //").
-    iIntros "!# %Φ' %vs' HΓ₁ HΦ'".
-    rewrite HcpyΓ₁. iDestruct "HΓ₁" as "#HΓ₁".
-    simpl. ewp_pure_steps. iApply "HΦ'". iLöb as "IH".
-    iSplitL; last done.
-    iIntros (w ws) "!# _ Hτ". rewrite env_dom_nil /=. ewp_pure_steps. 
-    rewrite delete_commute -subst_map_insert -delete_insert_ne; last done.
-    rewrite -subst_map_insert /= !subst_map_ctx_lambda.
-    destruct Δ₁ as [|[z ι] Δ₁'] eqn:HeqΔ.
-    - replace Δ₂ with ([] : env Σ) by 
-        (symmetry; apply (map_eq_nil fst); by apply list_nil_subseteq). 
-      rewrite !env_dom_nil /= !delete_list_nil insert_commute; last done.
-      rewrite lookup_insert lookup_delete. ewp_pure_steps.
-      iSplitL; last done.
-      iIntros (??) "_ -> /=". rewrite env_dom_nil /=.
-      ewp_pure_steps. iApply (ewp_bind [AppRCtx _]); first done.
-      replace ([] : list string) with (env_dom ([] : env Σ)) by done.
-      set f' := (rec: f x <> :=
-                  let: f := lambdas_norm f x (env_dom []) f in
-                  subst_map (delete f (delete f (delete x vs'))) e)%V.
-      rewrite -(subst_map_empty (lambdas_norm _ _ _ _ )).
-      iApply (sem_typed_lambdas_norm [] [] [] []  with "[] []"); 
-        [done|done|done|done| |done|].
-      { rewrite /f'. iIntros (Φ'' ?) "!# _ HΦ'' /=". ewp_pure_steps.
-        iApply "HΦ''". iDestruct "IH" as "[$ _]". }
-      iIntros (u) "[#Hτκ _] /=". ewp_pure_steps. 
-      rewrite -subst_map_insert insert_insert.
-      iApply ("He" with "[Hτ]"); last (iIntros (?) "[$ $] //").
-      solve_env. by do 2 (rewrite -env_sem_typed_insert; last done). 
-    - rewrite {4}env_dom_cons. iSimpl. ewp_pure_steps. iSplitL; last done.
-      rewrite !lookup_delete_not_elem; try done.
-      rewrite insert_commute; last done. rewrite lookup_insert lookup_delete.
-      rewrite !delete_list_commute delete_idemp delete_insert_delete.
-      iIntros (u us) "HΔ₁ -> /=". 
-      iApply (ewp_bind [AppLCtx _]); first done.
-      iApply (ewp_app_mult with "HΔ₁"). iIntros "HΔ₁ /=".
-      ewp_pure_steps. iApply (ewp_bind [AppRCtx _]); first done.
-      set f' := (rec: f x :=
-                    λ*λ: env_dom ((z, ι)%core :: Δ₁'), <>,
-                    (let: f := lambdas_norm f x (env_dom ((z, ι)%core :: Δ₁')) f in
-                    subst_map
-                      (delete (env_dom ((z, ι)%core :: Δ₁')) (delete f (delete x vs'))) e))%V.
-      replace (lambdas_norm f x (env_dom ((z,ι) :: Δ₁')) f') with
-              (subst_map us (lambdas_norm f x (env_dom ((z,ι) :: Δ₁')) f')) by done.
-      iApply (sem_typed_lambdas_norm _ _ ((z,ι) :: Δ₁') Δ₂ with "[] HΔ₁"); try done.
-      { iIntros (Φ'' ?) "!# HΔ₁ HΦ'' /=". rewrite /f'. ewp_pure_steps.
-        iApply "HΦ''". iSplitR "HΔ₁"; last done.
-        iDestruct "IH" as "[$ _]". }
-      iIntros (?) "[Hτκ HΔ₁] /=". ewp_pure_steps.
-      rewrite -subst_map_insert subst_map_union.
-      iApply ("He" with "[Hτ Hτκ HΔ₁]"). 
-      + iExists w. iFrame. iSplit.
-        { iPureIntro. apply lookup_union_Some_l.
-          rewrite delete_insert_ne; last done.
-          rewrite lookup_delete_not_elem; last done.
-          apply lookup_insert. }
-        iExists v. iFrame. iSplit.
-        { iPureIntro. rewrite lookup_union_r; [apply lookup_insert|].
-          by rewrite -delete_list_commute lookup_delete. }
-        rewrite app_comm_cons env_sem_typed_app. iSplitL "HΔ₁".
-        { rewrite -env_sem_typed_delete_union; last done.
-          rewrite -env_sem_typed_insert; last done.
-          by rewrite -env_sem_typed_difference_delete. }
-        iApply env_sem_typed_union.
-        rewrite -env_sem_typed_delete_disjoint; last done.
-        rewrite -env_sem_typed_delete; last done.
-        by rewrite -env_sem_typed_insert. 
-      + iIntros (?) "[$ HΔ₂]".
-        rewrite -env_sem_typed_delete_union; last done.
-        assert (f ∉ env_dom Δ₂).
-        { intros ?. apply H1. by eapply (elem_of_subseteq (env_dom Δ₂)); done. }
-        rewrite -env_sem_typed_insert; last done.
-        by iApply env_sem_typed_difference_delete.
+    ewp_pure_steps. iFrame.
+    iIntros (w) "Hτ". 
+    ewp_pure_steps. rewrite subst'_subst_map_insert.
+    iApply (ewp_pers_mono with "[Hτ HΓ₁]"); [iApply "He"|iIntros "!# % [$ _] //="].
+    destruct x; solve_env. 
   Qed.
 
-  Lemma sem_typed_ufun Γ₁ Γ₂ f x e τ ρ κ:
-    x ∉ (env_dom Γ₁) → f ∉ (env_dom Γ₁) → match f with BNamed f => BNamed f ≠ x | BAnon => True end →
+  Lemma sem_typed_ufun Γ₁ Γ₂ f x e τ ρs κ:
+    x ∉ (env_dom Γ₁) → f ∉ (env_dom Γ₁) → 
+    match f with BNamed f => BNamed f ≠ x | BAnon => True end →
     copy_env Γ₁ →
-    (x, τ) ::? (f, τ -{ ρ }-> κ) ::? Γ₁ ⊨ e : ρ : κ ⊨ [] -∗
-    Γ₁ ++ Γ₂ ⊨ (rec: f x :=  e) : ⟨⟩ : (τ -{ ρ }-> κ) ⊨ Γ₂.
+    (x, τ) ::? (f, τ -{ ρs }-> κ) ::? Γ₁ ⊨ e : ρs : κ ⊨ [] -∗
+    Γ₁ ++ Γ₂ ⊨ (rec: f x := e) : ⟨⟩ : (τ -{ ρs }-> κ) ⊨ Γ₂.
   Proof.
-    iIntros (??? HcpyΓ₁) "#He !# %Φ %vs HΓ₁₂ HΦ //=".
+    iIntros (??? HcpyΓ₁) "#He !# %vs HΓ₁₂ //=".
     ewp_pure_steps.
-    rewrite env_sem_typed_app. iApply "HΦ". 
-    iDestruct "HΓ₁₂" as "[HΓ₁ $]".
+    rewrite env_sem_typed_app. iDestruct "HΓ₁₂" as "[HΓ₁ $]".
     rewrite HcpyΓ₁. iDestruct "HΓ₁" as "#HΓ₁".
     iLöb as "IH".
-    iIntros (w ws) "!# _ Hτ". rewrite env_dom_nil /=. 
+    iIntros "!# %w  Hτ". 
     ewp_pure_steps. destruct f; destruct x; simpl.
-    - iApply ("He" with "HΓ₁ []").
-      iIntros (v) "[Hκ _] {$Hκ}".
+    - iApply ewp_pers_mono; [by iApply "He"|iIntros "!# % [$ _] //="].
     - rewrite -subst_map_insert. 
-      iApply ("He" with "[HΓ₁ Hτ] []"); first solve_env. 
-      iIntros (v) "//= [$ _]".
+      iApply (ewp_pers_mono with "[Hτ]"); [iApply "He"; solve_env|iIntros "!# % [$ _] //="].
     - rewrite -subst_map_insert.
-      iApply ("He" with "[HΓ₁ Hτ] []"); first solve_env.
-      iIntros (v) "//= [$ _]".
+      iApply (ewp_pers_mono with "[Hτ]"); [iApply "He"; solve_env|iIntros "!# % [$ _] //="].
     - assert (s ≠ s0) by (intros ?; simplify_eq).
       rewrite subst_subst_ne; last done.
       rewrite -subst_map_insert.
       rewrite -delete_insert_ne; last done. 
       rewrite -subst_map_insert.
-      iApply ("He" with "[Hτ] []"); first solve_env.
-      + by do 2 (rewrite -env_sem_typed_insert; last done).
-      + iIntros (v) "[$ _]". 
+      iApply (ewp_pers_mono with "[Hτ]"); [iApply "He"; solve_env|iIntros "!# % [$ _] //="].
+      by do 2 (rewrite -env_sem_typed_insert; last done).
   Qed.
 
-  Lemma sem_typed_ufun_poly_rec Γ₁ Γ₂ f x e τ ρ κ:
-    x ∉ (env_dom Γ₁) → f ∉ (env_dom Γ₁) → match x with BNamed x => BNamed x ≠ f | BAnon => True end →
+  Lemma sem_typed_ufun_poly_rec Γ₁ Γ₂ f x e τ ρs κ:
+    x ∉ (env_dom Γ₁) → f ∉ (env_dom Γ₁) → 
+    match x with BNamed x => BNamed x ≠ f | BAnon => True end →
     copy_env Γ₁ →
-    (∀ ι, (x, τ ι) ::? (f, ∀T: α,, τ α -{ ρ α }-> κ α) ::? Γ₁ ⊨ e : ρ ι : κ ι ⊨ []) -∗
-    Γ₁ ++ Γ₂ ⊨ (rec: f <> := λ: x, e) : ⟨⟩ : (∀T: α,, τ α -{ ρ α }-> κ α) ⊨ Γ₂.
+    (∀ ι, (x, τ ι) ::? (f, ∀T: α,, τ α -{ ρs α }-> κ α) ::? Γ₁ ⊨ e : ρs ι : κ ι ⊨ []) -∗
+    Γ₁ ++ Γ₂ ⊨ (rec: f <> := λ: x, e) : ⟨⟩ : (∀T: α,, τ α -{ ρs α }-> κ α) ⊨ Γ₂.
   Proof.
-    iIntros (??? HcpyΓ₁) "#He !# %Φ %vs HΓ₁₂ HΦ //=".
-    ewp_pure_steps.
-    rewrite env_sem_typed_app. iApply "HΦ". 
+    iIntros (??? HcpyΓ₁) "#He !# %vs HΓ₁₂ //=".
+    ewp_pure_steps. rewrite env_sem_typed_app. 
     iDestruct "HΓ₁₂" as "[HΓ₁ $]".
     rewrite HcpyΓ₁. iDestruct "HΓ₁" as "#HΓ₁".
     iLöb as "IH".
     iIntros (α) "!#". ewp_pure_steps.
     destruct f; destruct x; simpl; 
-    ewp_pure_steps; iIntros (v ?) "!# _ Hτ";
-    rewrite env_dom_nil /=; ewp_pure_steps.
-    - iApply ("He" with "HΓ₁ []").
-      iIntros (?) "[$ _]".
+    ewp_pure_steps; iIntros (v) "!# Hτ"; ewp_pure_steps.
+    - iApply ewp_pers_mono; first (by iApply "He").  
+      iIntros "!# % [$ _] //=".
     - rewrite -subst_map_insert. 
-      iApply ("He" with "[HΓ₁ Hτ] []"); first solve_env. 
-      iIntros (?) "//= [$ _]".
+      iApply (ewp_pers_mono with "[Hτ]"); first (iApply "He"; solve_env).  
+      iIntros "!# % [$ _] //=".
     - rewrite -subst_map_insert.
-      iApply ("He" with "[HΓ₁ Hτ] []"); first solve_env.
-      iIntros (?) "//= [$ _]".
+      iApply (ewp_pers_mono with "[Hτ]"); first (iApply "He"; solve_env).  
+      iIntros "!# % [$ _] //=".
     - assert (s ≠ s0) by (intros ?; simplify_eq).
       rewrite decide_True; last auto.
       rewrite subst_subst_ne; last done.
       rewrite -subst_map_insert.
       rewrite -delete_insert_ne; last done. 
       rewrite -subst_map_insert.
-      iApply ("He" with "[Hτ] []"); first solve_env.
+      iApply (ewp_pers_mono with "[Hτ]"); first (iApply "He"; solve_env).  
       + by do 2 (rewrite -env_sem_typed_insert; last done).
-      + iIntros (?) "[$ _]". 
+      + iIntros "!# % [$ _] //=".
   Qed.
 
-  Lemma sem_typed_sufun_mult Γ₁ Γ₂ Δ₁ Δ₂ x e τ ρ κ:
-    x ∉ (env_dom Γ₁) → x ∉ (env_dom Δ₁) → x ∉ (env_dom Γ₂) →
-    env_dom Δ₂ ⊆ env_dom Δ₁ →
-    env_dom Γ₁ ## env_dom Δ₁ →
-    (x, τ) ::? Δ₁ ++ Γ₁ ⊨ e : ρ : κ ⊨ Δ₂ ++ Γ₁ -∗
-    Γ₁ ++ Γ₂ ⊨ (λ*λ: env_dom Δ₁, x, e) : ⟨⟩ : (τ >-{ ρ ; Δ₁ ; Δ₂ }-∘ κ) ⊨ Γ₂.
-  Proof.
-    iIntros (?????) "#He !# %Φ %vs HΓ₁₂ HΦ /=".
-    iDestruct (env_sem_typed_app with "HΓ₁₂") as "[HΓ₁ HΓ₂]".
-    iApply (ewp_mono _ _ (λ v, (τ >-{ ρ; Δ₁; Δ₂ }-∘ κ) v ∗ env_sem_typed Γ₂ vs) 
-            with "[HΓ₁ HΓ₂]"); [|iIntros (w); iIntros "? !>"; by iApply "HΦ"].
-    iApply (ewp_frame_r with "[HΓ₁] HΓ₂").
-    rewrite subst_map_ctx_lambda. iSimpl.
-    destruct Δ₁ as [|[z ι] Δ₁'].
-    - rewrite env_dom_nil delete_list_nil. iSimpl. ewp_pure_steps.
-      replace Δ₂ with ([] : env Σ) 
-          by (symmetry; apply (map_eq_nil fst); by apply list_nil_subseteq). 
-      iLöb as "IH". iApply sem_ty_suarr_unfold.
-      iIntros (u ws) "_ Hτ /=". rewrite env_dom_nil. iSimpl.
-      ewp_pure_steps. destruct x as [|x]. iSimpl.
-      + iApply ("He" with "HΓ₁"). iIntros "%v [Hκ HΓ₁] {$Hκ}".
-        iSpecialize ("IH" with "HΓ₁"). solve_env.
-      + iSimpl. rewrite -subst_map_insert.
-        iApply ("He" with "[Hτ HΓ₁]"); iSimpl; first solve_env. 
-        iIntros "%v [Hκ HΓ₁] {$Hκ}".
-        rewrite -env_sem_typed_insert; last done.
-        iSpecialize ("IH" with "HΓ₁"); solve_env.
-    - rewrite env_dom_cons /=. ewp_pure_steps.
-      iLöb as "IH". iApply sem_ty_suarr_unfold.
-      iIntros (u ws) "HΔ₁ Hτ". 
-      iApply (ewp_bind [AppLCtx _]); first done. 
-      ewp_bottom.
-      set Δ₁ := (z, ι) :: Δ₁'.
-      set e' := subst_map (binder_delete x (delete (z :: env_dom Δ₁') vs)) e.
-      iApply (ewp_app_mult with "[HΔ₁]"); first done. iIntros "HΔ₁".
-      simpl. ewp_pure_steps.
-      rewrite /e' env_dom_cons subst_map_union -binder_delete_union subst'_subst_map_insert -(env_dom_cons _ ι).
-      iApply ("He" with "[HΔ₁ Hτ HΓ₁]"); destruct x as [|x]. 
-      + rewrite app_comm_cons env_sem_typed_app -/Δ₁. iSimpl.
-        iSplitL "HΔ₁".
-        { rewrite (env_sem_typed_difference_delete Δ₁); last reflexivity. 
-          by rewrite (env_sem_typed_delete_union Δ₁); last reflexivity. }
-        { rewrite (env_sem_typed_delete_disjoint Γ₁ Δ₁); last done. 
-        by iApply env_sem_typed_union. }
-      + iExists u. iSplitL ""; first (iPureIntro; apply lookup_insert). iFrame.
-        rewrite app_comm_cons -/Δ₁.
-        rewrite -(env_sem_typed_insert (Δ₁ ++ Γ₁) _ x u);
-          last (rewrite env_dom_app; by eapply not_elem_of_app).
-        rewrite env_sem_typed_app.
-        rewrite (env_sem_typed_difference_delete Δ₁); last reflexivity.
-        rewrite (env_sem_typed_delete_union Δ₁); last reflexivity. iFrame.
-        rewrite (env_sem_typed_delete_disjoint Γ₁ Δ₁); last done. 
-        by iApply (env_sem_typed_union Γ₁). 
-      + iIntros (w) "[$ HΔ₂Γ₁] /=". 
-        iDestruct (env_sem_typed_app with "HΔ₂Γ₁") as "[HΔ₂ HΓ₁]".
-        rewrite -(env_sem_typed_delete_union Δ₂ Δ₁); last done. 
-        rewrite -(env_sem_typed_difference_delete Δ₂ Δ₁); last done. iFrame. 
-        iApply "IH".
-        rewrite (env_sem_typed_union_difference_delete Γ₁ Δ₁); last done.
-        by iApply env_sem_typed_delete_disjoint.
-      + iIntros (w) "[$ HΔ₂Γ₁] /=". 
-        iDestruct (env_sem_typed_app with "HΔ₂Γ₁") as "[HΔ₂ HΓ₁]".
-        assert (x ∉ env_dom Δ₂).
-        { intros ?. apply H0. 
-          destruct (elem_of_subseteq (env_dom Δ₂) (env_dom Δ₁)) as [H' _]. by apply H'. }
-        do 2 (rewrite -env_sem_typed_insert; last done).
-        rewrite -(env_sem_typed_delete_union Δ₂ Δ₁); last done. 
-        rewrite -(env_sem_typed_difference_delete Δ₂ Δ₁); last done. iFrame. 
-        iApply "IH".
-        rewrite (env_sem_typed_union_difference_delete Γ₁ Δ₁); last done.
-        by iApply env_sem_typed_delete_disjoint.
-  Qed.
-
-  Lemma sem_typed_sufun Γ₁ Γ₂ x e τ ρ κ:
-    x ∉ (env_dom Γ₁) → x ∉ (env_dom Γ₂) →
-    (x, τ) ::? Γ₁ ⊨ e : ρ : κ ⊨ Γ₁ -∗
-    Γ₁ ++ Γ₂ ⊨ (λ: x, e) : ⟨⟩ : (τ >-{ ρ }-∘ κ) ⊨ Γ₂.
-  Proof.
-    intros ??.
-    rewrite [(λ: x, _)%E](@ctx_lambda_env_dom_nil Σ).
-    iApply (sem_typed_sufun_mult _ _ [] []); solve_sidecond.
-  Qed.
-
-  Lemma sem_typed_app_mult Γ₁ Γ₂ Γ₃ Δ₁ Δ₂ e₁ e₂ τ ρ κ: 
-    Γ₂ ⊨ e₁ : ρ : (τ -{ ρ ; Δ₁ ; Δ₂ }-∘ κ) ⊨ Γ₃ -∗
-    Γ₁ ⊨ e₂ : ρ : τ ⊨ Δ₁ ++ Γ₂ -∗
-    Γ₁ ⊨ (e₁ <_ map Var (env_dom Δ₁) _> e₂) : ρ : κ ⊨ Δ₂ ++ Γ₃.
-  Proof.
-    iIntros "#He₁ #He₂ !# %Φ %vs HΓ₁ HΦ //=".
-    rewrite subst_map_app_mult map_map.
-    iApply (ewp_bind [AppRCtx _]); first done.
-    iApply ("He₂" with "HΓ₁").
-    iIntros (v) "[Hτ HΔ₁Γ₂]". 
-    iDestruct (env_sem_typed_app with "HΔ₁Γ₂") as "[HΔ₁ HΓ₂]".
-    replace (λ (x : string), subst_map vs x) with (subst_map vs ∘ Var) by done.
-    iDestruct (subst_map_var with "HΔ₁") as "[%ws %Hrw]". rewrite Hrw /=.
-    assert (Hfold : ∀ e, (e <_ map Val ws _> v)%E = (e <_ map Val (ws ++ [v]) _>)%E).
-    { clear - ws v. induction ws; first done. simpl. intros e. by rewrite IHws. }
-    rewrite Hfold.
-    iApply ewp_bind_app_mult. 
-    iApply ("He₁" with "HΓ₂"). simpl.
-    iIntros (w) "[Hτκw HΓ₃] //=". rewrite -Hfold -Hrw.
-    iApply (ewp_mono with "[Hτκw HΔ₁ Hτ]").
-    { iApply ("Hτκw" $! v vs with "HΔ₁ Hτ"). }
-    iIntros (u) "[Hκ HΔ₂] !>". iApply "HΦ". rewrite env_sem_typed_app. iFrame.
-  Qed.
-  
-  Lemma sem_typed_app Γ₁ Γ₂ Γ₃ e₁ e₂ τ ρ κ: 
-    Γ₂ ⊨ e₁ : ρ : (τ -{ ρ }-∘ κ) ⊨ Γ₃ -∗
-    Γ₁ ⊨ e₂ : ρ : τ ⊨ Γ₂ -∗
-    Γ₁ ⊨ (e₁ e₂) : ρ : κ ⊨ Γ₃.
-  Proof.
-    rewrite {2} [e₁](@app_mult_env_dom_nil Σ) - {2} (app_nil_l Γ₃).
-    iApply sem_typed_app_mult.
-  Qed.
-
-  Lemma sem_typed_suapp_mult Γ₁ Γ₂ Δ₁ Δ₂ f e₂ τ ρ κ: 
-    Γ₁ ⊨ e₂ : ρ : τ ⊨ (f, τ >-{ ρ ; Δ₁ ; Δ₂ }-∘ κ) :: Δ₁ ++ Γ₂ -∗
-    Γ₁ ⊨ (f <_ map Var (env_dom Δ₁) _> e₂) : ρ : κ ⊨ (f, τ >-{ ρ ; Δ₁ ; Δ₂  }-∘ κ) :: Δ₂ ++ Γ₂. 
-  Proof.
-    iIntros "#He₂ !# %Φ %vs HΓ₁ HΦ /=".
-    rewrite subst_map_app_mult. simpl.
-    iApply (ewp_bind ([AppRCtx _])); first done.
-    iApply ("He₂" with "HΓ₁").
-    iIntros (v) "/= [Hτ [%w (%Hrw & Hw & HΓ₂)]] /=". rewrite Hrw.
-    iDestruct (env_sem_typed_app with "HΓ₂") as "[HΔ₁ HΓ₂]".
-    rewrite sem_ty_suarr_unfold.
-    iApply (ewp_mono with "[Hτ HΔ₁ Hw]").
-    - iSpecialize ("Hw" $! v vs with "HΔ₁ Hτ").
-      rewrite -map_map. iApply "Hw". 
-    - iIntros (u) "[Hκ [HΔ₂ Hw]] !>". iApply "HΦ". iFrame.
-      iExists w. rewrite env_sem_typed_app. by iFrame.
-  Qed.
-
-  Lemma sem_typed_suapp Γ₁ Γ₂ f e₂ τ ρ κ: 
-    Γ₁ ⊨ e₂ : ρ : τ ⊨ (f, τ >-{ ρ }-∘ κ) :: Γ₂ -∗
-    Γ₁ ⊨ (f e₂) : ρ : κ ⊨ (f, τ >-{ ρ }-∘ κ) :: Γ₂. 
-  Proof.
-    rewrite [Var f](@app_mult_env_dom_nil Σ) - {2} (app_nil_l Γ₂).
-    iApply sem_typed_suapp_mult.
-  Qed.
-
-  Lemma sem_typed_let Γ₁ Γ₂ Γ₃ x e₁ e₂ τ ρ κ: 
+  Lemma sem_typed_let Γ₁ Γ₂ Γ₃ x e₁ e₂ τ ρs κ: 
     x ∉ (env_dom Γ₂) → x ∉ (env_dom Γ₃) →
-    Γ₁ ⊨ e₁ : ρ : τ ⊨ Γ₂ -∗
-    (x, τ) :: Γ₂ ⊨ e₂ : ρ : κ ⊨ Γ₃ -∗
-    Γ₁ ⊨ (let: x := e₁ in e₂) : ρ : κ ⊨ Γ₃.
+    Γ₁ ⊨ e₁ : ρs : τ ⊨ Γ₂ -∗
+    (x, τ) :: Γ₂ ⊨ e₂ : ρs : κ ⊨ Γ₃ -∗
+    Γ₁ ⊨ (let: x := e₁ in e₂) : ρs : κ ⊨ Γ₃.
   Proof.
-    iIntros (??) "#He₁ #He₂ !# %Φ %vs HΓ₁ HΦ /=".
-    iApply (ewp_bind ([AppRCtx _])); first done.
-    iApply ("He₁" with "HΓ₁").
-    iIntros (v) "[Hτ HΓ₂] /=". ewp_pure_steps.
+    iIntros (??) "#He₁ #He₂ !# %vs HΓ₁ /=".
+    iApply (ewp_bind ([AppRCtx _])); first done. simpl.
+    iApply (ewp_pers_mono with "[HΓ₁]"); first (by iApply "He₁").
+    iIntros "!# % [Hτ HΓ₂] !> /=". ewp_pure_steps.
     rewrite -subst_map_insert.
-    iApply ("He₂" with "[Hτ HΓ₂]"); first solve_env.
-    iIntros (w) "[Hκ HΓ₃]". iApply "HΦ". iFrame.
-    by iApply env_sem_typed_insert.
+    iApply (ewp_pers_mono with "[Hτ HΓ₂]"); first (iApply "He₂"; solve_env).
+    iIntros "!# % [Hτκ HΓ₃] !> /=".
+    solve_env.
   Qed.
 
-  Lemma sem_typed_seq Γ₁ Γ₂ Γ₃ e₁ e₂ τ ρ κ: 
-    Γ₁ ⊨ e₁ : ρ : τ ⊨ Γ₂ -∗
-    Γ₂ ⊨ e₂ : ρ : κ ⊨ Γ₃ -∗
-    Γ₁ ⊨ (e₁ ;; e₂) : ρ : κ ⊨ Γ₃.
+  Lemma sem_typed_app Γ₁ Γ₂ Γ₃ e₁ e₂ τ ρs κ: 
+    copy_env Γ₃ →
+    Γ₂ ⊨ e₁ : ⟨ρs.1,⟩ : (τ -{ ρs }-∘ κ) ⊨ Γ₃ -∗
+    Γ₁ ⊨ e₂ : ρs : τ ⊨ Γ₂ -∗
+    Γ₁ ⊨ (e₁ e₂) : ρs : κ ⊨ Γ₃.
   Proof.
-    iIntros "#He₁ #He₂ !# %Φ %vs HΓ₁ HΦ /=".
-    iApply (ewp_bind ([AppRCtx _])); first done.
-    iApply ("He₁" with "HΓ₁").
-    iIntros (v) "[Hτ HΓ₂] /=". ewp_pure_steps.
-    iApply ("He₂" with "HΓ₂").
-    iIntros (w) "[Hκ HΓ₃]". iApply "HΦ". iFrame.
+    iIntros (Hcpy) "#He₁ #He₂ !# %vs HΓ₁ /=".
+    iApply (ewp_bind [AppRCtx _]); first done.
+    iApply (ewp_pers_mono with "[HΓ₁]"); first (by iApply "He₂").
+    iIntros "!# % [Hτ HΓ₂] !> /=".
+    iApply (ewp_bind [AppLCtx _]); first done.
+    iApply ewp_ms_prot_mono; [iApply sig_le_nil|].
+    iApply (ewp_mono with "[HΓ₂]"); first (by iApply "He₁").
+    iIntros "% [Hτκ HΓ₃] !> /=".
+    rewrite {1}Hcpy. iDestruct "HΓ₃" as "#HΓ₃".
+    iApply (ewp_pers_mono with "[Hτ Hτκ]"); first (by iApply "Hτκ").
+    iIntros "!# % $ !> //=".
   Qed.
 
-  Lemma sem_typed_pair Γ₁ Γ₂ Γ₃ e₁ e₂ τ ρ κ: 
-    Γ₂ ⊨ e₁ : ρ : τ ⊨ Γ₃ -∗
-    Γ₁ ⊨ e₂ : ρ : κ ⊨ Γ₂ -∗
-    Γ₁ ⊨ (e₁,e₂) : ρ : (τ × κ) ⊨ Γ₃.
+  Lemma sem_typed_app_alt Γ₁ Γ₂ Γ₃ (x₁ x₂ : string) e₁ e₂ τ ρs κ: 
+    x₂ ∉ env_dom Γ₂ → x₂ ∉ env_dom Γ₃ → 
+    x₁ ∉ env_dom Γ₃ → x₁ ≠ x₂ →
+    copy_ty τ → copy_env Γ₃ →
+    Γ₂ ⊨ e₁ : ρs : (τ -{ ρs }-∘ κ) ⊨ Γ₃ -∗
+    Γ₁ ⊨ e₂ : ρs : τ ⊨ Γ₂ -∗
+    Γ₁ ⊨ (let: x₂ := e₂ in let: x₁ := e₁ in (x₁ x₂)) : ρs : κ ⊨ Γ₃.
   Proof.
-    iIntros "#He₁ #He₂ !# %Φ %vs HΓ₁ HΦ //=".
+    iIntros (???? Hcpyτ HcpyΓ₃) "#He₁ #He₂".
+    iApply (sem_typed_let _ Γ₂); solve_sidecond.
+    iApply (sem_typed_let _ ((x₂, τ) :: Γ₃)); solve_sidecond.
+    { iApply sem_typed_frame_ms; first done. iApply "He₁". }
+    iApply (sem_typed_app _ ((x₁, τ -{ ρs }-∘ κ) :: Γ₃)); first done.
+    { iApply sem_typed_sub_nil. iApply sem_typed_var. }
+    iApply sem_typed_swap_second.
+    iApply sem_typed_sub_nil. iApply sem_typed_var.
+  Qed.
+
+  Lemma sem_typed_app_alt' Γ₁ Γ₂ Γ₃ (x₁ x₂ : string) e₁ e₂ τ ρs κ: 
+    x₂ ∉ env_dom Γ₂ → x₂ ∉ env_dom Γ₃ → 
+    x₁ ∉ env_dom Γ₃ → x₁ ≠ x₂ →
+    Γ₂ ⊨ e₁ : ⟨ρs.1,⟩ : (τ -{ ⟨ρs.1,⟩ }-∘ κ) ⊨ Γ₃ -∗
+    Γ₁ ⊨ e₂ : ρs : τ ⊨ Γ₂ -∗
+    Γ₁ ⊨ (let: x₂ := e₂ in let: x₁ := e₁ in (x₁ x₂)) : ρs : κ ⊨ Γ₃.
+  Proof.
+    iIntros (????) "#He₁ #He₂".
+    iApply (sem_typed_let _ Γ₂); solve_sidecond.
+    iApply (sem_typed_let _ ((x₂, τ) :: Γ₃)); solve_sidecond.
+    { iApply sem_typed_sub_sig. 
+        { apply sigs_le_comp; [apply sig_le_refl|apply sig_le_nil]. }
+      iApply sem_typed_frame_os; first done. }
+    iApply sem_typed_swap_env_singl. rewrite -app_comm_cons.
+    iApply sem_typed_swap_env_singl. rewrite -app_assoc.
+    rewrite - {3} (app_nil_r Γ₃).
+    iApply sem_typed_sub_sig. 
+    { apply sigs_le_comp; [apply sig_le_refl|apply sig_le_nil]. }
+    iApply sem_typed_frame_env_os. simpl.
+    iApply (sem_typed_app _ [(x₁, τ -{ ⟨ρs.1,⟩ }-∘ κ)]); first solve_copy.
+    { iApply sem_typed_sub_nil. iApply sem_typed_var. }
+    iApply sem_typed_swap_second.
+    iApply sem_typed_sub_nil. iApply sem_typed_var. 
+  Qed.
+
+  Lemma sem_typed_seq Γ₁ Γ₂ Γ₃ e₁ e₂ τ ρs κ: 
+    Γ₁ ⊨ e₁ : ρs : τ ⊨ Γ₂ -∗
+    Γ₂ ⊨ e₂ : ρs : κ ⊨ Γ₃ -∗
+    Γ₁ ⊨ (e₁ ;; e₂) : ρs : κ ⊨ Γ₃.
+  Proof.
+    iIntros "#He₁ #He₂ !# %vs HΓ₁ /=".
+    iApply (ewp_bind ([AppRCtx _])); first done. simpl.
+    iApply (ewp_pers_mono with "[HΓ₁]"); first (by iApply "He₁").
+    iIntros "!# % [Hτ HΓ₂] !> /=". ewp_pure_steps.
+    iApply (ewp_pers_mono with "[Hτ HΓ₂]"); first (by iApply "He₂").
+    iIntros "!# % [Hτκ HΓ₃] !> /=". iFrame.
+  Qed.
+
+  Lemma sem_typed_pair Γ₁ Γ₂ Γ₃ e₁ e₂ τ ρs κ: 
+    Γ₂ ⊨ e₁ : ⟨ρs.1,⟩ : τ ⊨ Γ₃ -∗
+    Γ₁ ⊨ e₂ : ρs : κ ⊨ Γ₂ -∗
+    Γ₁ ⊨ (e₁,e₂) : ρs : (τ × κ) ⊨ Γ₃.
+  Proof.
+    iIntros "#He₁ #He₂ !# %vs HΓ₁ //=".
     iApply (ewp_bind ([PairRCtx (subst_map vs e₁)])); first done.
-    iApply ("He₂" with "HΓ₁").
-    iIntros (v) "[Hτv HΓ₂] //=".
+    iApply (ewp_pers_mono with "[HΓ₁]"); first (by iApply "He₂").
+    iIntros "!# % [Hτ HΓ₂] !> /=".
     iApply (ewp_bind ([PairLCtx v])); first done.
-    iApply ("He₁" with "HΓ₂").
-    iIntros (w) "[Hκw HΓ₃] //=". ewp_pure_steps.
-    iApply "HΦ". iFrame. iExists w, v. iFrame. by iPureIntro.
+    iApply ewp_ms_prot_mono; [iApply sig_le_nil|].
+    iApply (ewp_mono with "[HΓ₂]"); first (by iApply "He₁").
+    iIntros (w) "[Hκw HΓ₃] //= !>". ewp_pure_steps.
+    solve_env.
   Qed.
   
-  Lemma sem_typed_pair_elim Γ₁ Γ₂ Γ₃ x₁ x₂ e₁ e₂ τ ρ κ ι: 
+  Lemma sem_typed_pair_ms Γ₁ Γ₂ Γ₃ (x₁ x₂ : string) e₁ e₂ τ ρs κ: 
+    x₂ ∉ env_dom Γ₂ → x₂ ∉ env_dom Γ₃ → x₁ ∉ env_dom Γ₃ → x₁ ≠ x₂ →
+    copy_ty κ →
+    Γ₂ ⊨ e₁ : ρs : τ ⊨ Γ₃ -∗
+    Γ₁ ⊨ e₂ : ρs : κ ⊨ Γ₂ -∗
+    Γ₁ ⊨ (let: x₂ := e₂ in let: x₁ := e₁ in (x₁,x₂)) : ρs : (τ × κ) ⊨ Γ₃.
+  Proof.
+    iIntros (???? Hcpy) "#He₁ #He₂".
+    iApply (sem_typed_let _ Γ₂); solve_sidecond.
+    iApply (sem_typed_let _ ((x₂, κ) :: Γ₃)); solve_sidecond.
+    { iApply sem_typed_frame_ms; first done. iApply "He₁". }
+    iApply sem_typed_sub_nil.
+    iApply (sem_typed_pair _ ((x₁, τ) :: Γ₃)); [iApply sem_typed_var|].
+    iApply sem_typed_swap_second.
+    iApply sem_typed_var.
+  Qed.
+
+  Lemma sem_typed_pair_elim Γ₁ Γ₂ Γ₃ x₁ x₂ e₁ e₂ τ ρs κ ι: 
     x₁ ∉ (env_dom Γ₂) → x₂ ∉ (env_dom Γ₂) →
     x₁ ∉ (env_dom Γ₃) → x₂ ∉ (env_dom Γ₃) →
     x₁ ≠ x₂ →
-    Γ₁ ⊨ e₁ : ρ : (τ × κ) ⊨ Γ₂ -∗
-    (x₁, τ) :: (x₂, κ) :: Γ₂ ⊨ e₂ : ρ : ι ⊨ Γ₃ -∗
-    Γ₁ ⊨ (let: (x₁, x₂) := e₁ in e₂) : ρ : ι ⊨ Γ₃.
+    Γ₁ ⊨ e₁ : ρs : (τ × κ) ⊨ Γ₂ -∗
+    (x₁, τ) :: (x₂, κ) :: Γ₂ ⊨ e₂ : ρs : ι ⊨ Γ₃ -∗
+    Γ₁ ⊨ (let: (x₁, x₂) := e₁ in e₂) : ρs : ι ⊨ Γ₃.
   Proof.
-    iIntros (?????) "#He₁ #He₂ !# %Φ %vs HΓ₁ HΦ //=".
-    ewp_pure_steps.
+    iIntros (?????) "#He₁ #He₂ !# %vs HΓ₁ //=". ewp_pure_steps.
     set ex1x2 := (λ: x₁ x₂, subst_map (binder_delete x₂ 
                                       (binder_delete x₁ vs)) e₂)%V. 
     iApply (ewp_bind ([AppLCtx ex1x2; AppRCtx pair_elim])); first done.
-    iApply ("He₁" with "HΓ₁").
-    iIntros (v) "[Hτκv HΓ₂] //=". 
+    iApply (ewp_pers_mono with "[HΓ₁]"); first (by iApply "He₁").
+    iIntros "!# % [Hτκv HΓ₂] //= !>". 
     unfold pair_elim. ewp_pure_steps.
     iDestruct "Hτκv" as "(%v₁ & %v₂ & -> & Hτ & Hκ)".
     unfold ex1x2. ewp_pure_steps. 
     destruct (decide _) as [[]|[]]; [|split; [done|congruence]].
     rewrite delete_commute -subst_map_insert -delete_insert_ne; last congruence.
     rewrite -subst_map_insert.
-    iApply ("He₂" with "[Hτ Hκ HΓ₂]").
+    iApply (ewp_pers_mono with "[Hτ Hκ HΓ₂]"); first (iApply "He₂").
     - iExists v₁. iFrame. iSplitL "".
       { rewrite lookup_insert_ne; last done. by rewrite lookup_insert. }
       iExists v₂. iFrame; iSplitL ""; [by rewrite lookup_insert|].
       by do 2 (rewrite -env_sem_typed_insert; last done).
-    - iIntros (v) "[Hιv HΓ₃]". iApply "HΦ". iFrame.
+    - iIntros "!# % [Hιv HΓ₃]". iFrame.
       rewrite -(env_sem_typed_insert _ _ x₂ v₂); last done.
       by rewrite -(env_sem_typed_insert _ _ x₁ v₁).
   Qed.
   
-  Lemma sem_typed_left_inj Γ₁ Γ₂ e τ ρ κ: 
-    Γ₁ ⊨ e : ρ : τ ⊨ Γ₂ -∗
-    Γ₁ ⊨ InjL e : ρ : (τ + κ) ⊨ Γ₂.
+  Lemma sem_typed_left_inj Γ₁ Γ₂ e τ ρs κ: 
+    Γ₁ ⊨ e : ρs : τ ⊨ Γ₂ -∗
+    Γ₁ ⊨ InjL e : ρs : (τ + κ) ⊨ Γ₂.
   Proof.
-    iIntros "#He !# %Φ %vs HΓ₁ HΦ //=".
+    iIntros "#He !# %vs HΓ₁ //=".
     iApply (ewp_bind [InjLCtx]); first done.
-    iApply ("He" with "HΓ₁").
-    iIntros (v) "[Hv HΓ₂] //=".
-    ewp_pure_steps. iApply "HΦ".
+    iApply (ewp_pers_mono with "[HΓ₁]"); first (by iApply "He").
+    iIntros "!# % [Hτ HΓ₂] /= !>". ewp_pure_steps.
     iFrame. iExists v. iLeft. by iFrame.
   Qed.
 
-  Lemma sem_typed_right_inj Γ₁ Γ₂ e τ ρ κ: 
-    Γ₁ ⊨ e : ρ : κ ⊨ Γ₂ -∗
-    Γ₁ ⊨ InjR e : ρ : (τ + κ) ⊨ Γ₂.
+  Lemma sem_typed_right_inj Γ₁ Γ₂ e τ ρs κ: 
+    Γ₁ ⊨ e : ρs : κ ⊨ Γ₂ -∗
+    Γ₁ ⊨ InjR e : ρs : (τ + κ) ⊨ Γ₂.
   Proof.
-    iIntros "#He !# %Φ %vs HΓ₁ HΦ //=".
+    iIntros "#He !# %vs HΓ₁ //=".
     iApply (ewp_bind [InjRCtx]); first done.
-    iApply ("He" with "HΓ₁").
-    iIntros (v) "[Hv HΓ₂] //=".
-    ewp_pure_steps. iApply "HΦ".
+    iApply (ewp_pers_mono with "[HΓ₁]"); first (by iApply "He").
+    iIntros "!# % [Hκ HΓ₂] /= !>". ewp_pure_steps.
     iFrame. iExists v. iRight. by iFrame.
   Qed.
 
-  Lemma sem_typed_match Γ₁ Γ₂ Γ₃ e₁ x y e₂ e₃ τ ρ κ ι: 
+  Lemma sem_typed_match Γ₁ Γ₂ Γ₃ e₁ x y e₂ e₃ τ ρs κ ι: 
     x ∉ env_dom Γ₂ → x ∉ env_dom Γ₃ → y ∉ env_dom Γ₂ → y ∉ env_dom Γ₃ →
-    Γ₁ ⊨ e₁ : ρ : (τ + κ) ⊨ Γ₂ -∗
-    (x, τ) ::? Γ₂ ⊨ e₂ : ρ : ι ⊨ Γ₃ -∗
-    (y, κ) ::? Γ₂ ⊨ e₃ : ρ : ι ⊨ Γ₃ -∗
-    Γ₁ ⊨ match: e₁ with InjL x => e₂ | InjR y => e₃ end : ρ : ι ⊨ Γ₃.
+    Γ₁ ⊨ e₁ : ρs : (τ + κ) ⊨ Γ₂ -∗
+    (x, τ) ::? Γ₂ ⊨ e₂ : ρs : ι ⊨ Γ₃ -∗
+    (y, κ) ::? Γ₂ ⊨ e₃ : ρs : ι ⊨ Γ₃ -∗
+    Γ₁ ⊨ match: e₁ with InjL x => e₂ | InjR y => e₃ end : ρs : ι ⊨ Γ₃.
   Proof.
-    iIntros (????) "#He₁ #He₂ #He₃ !# %Φ %vs HΓ₁ HΦ //=".
+    iIntros (????) "#He₁ #He₂ #He₃ !# %vs HΓ₁ //=".
     iApply (ewp_bind [CaseCtx _ _]); first done.
-    iApply ("He₁" with "HΓ₁"). simpl.
-    iIntros (v) "[(%w & [(-> & Hτ)|(-> & Hκ)]) HΓ₂] //="; 
-      ewp_pure_steps.
+    iApply (ewp_pers_mono with "[HΓ₁]"); first (by iApply "He₁").
+    iIntros "!# %v [(%w & [(-> & Hτ)|(-> & Hκ)]) HΓ₂] //= !>"; ewp_pure_steps.
     - destruct x; simpl.
-      + iApply ("He₂" with "[HΓ₂ Hτ] [HΦ]"); [solve_env|eauto].
+      + iApply (ewp_pers_mono with "[HΓ₂ Hτ]"); [by iApply "He₂"|eauto].
       + rewrite -subst_map_insert.
-        iApply ("He₂" with "[HΓ₂ Hτ] [HΦ]"); [solve_env|].
-        iIntros (?) "[Hι HΓ₃]". iApply "HΦ". solve_env.
+        iApply (ewp_pers_mono with "[HΓ₂ Hτ]"); first (iApply "He₂"; solve_env).
+        iIntros "!# % [$ HΓ₃] //=". solve_env.
     - destruct y; simpl.
-      + iApply ("He₃" with "[HΓ₂ Hκ] [HΦ]"); [solve_env|eauto].
+      + iApply (ewp_pers_mono with "[HΓ₂ Hκ]"); [iApply "He₃"; solve_env|eauto].
       + rewrite -subst_map_insert.
-        iApply ("He₃" with "[HΓ₂ Hκ] [HΦ]"); [solve_env|].
-        iIntros (?) "[Hι HΓ₃]". iApply "HΦ". solve_env.
+        iApply (ewp_pers_mono with "[HΓ₂ Hκ]"); [iApply "He₃"; solve_env|].
+        iIntros "!# % [$ HΓ₃] //=". solve_env.
   Qed.
 
   Lemma sem_typed_none Γ₁ τ: 
@@ -793,91 +555,108 @@ Section compatibility.
     iIntros. iApply sem_typed_left_inj. iApply sem_typed_unit. 
   Qed.
 
-  Lemma sem_typed_some Γ₁ Γ₂ e ρ τ: 
-    Γ₁ ⊨ e : ρ : τ ⊨ Γ₂ -∗ 
-    Γ₁ ⊨ SOME e : ρ : Option τ ⊨ Γ₂.
+  Lemma sem_typed_some Γ₁ Γ₂ e ρs τ: 
+    Γ₁ ⊨ e : ρs : τ ⊨ Γ₂ -∗ 
+    Γ₁ ⊨ SOME e : ρs : Option τ ⊨ Γ₂.
   Proof.
     iIntros "He". iApply sem_typed_right_inj. iApply "He".
   Qed.
 
-  Lemma sem_typed_match_option Γ₁ Γ₂ Γ₃ e₁ x e₂ e₃ τ ρ κ ι: 
-    x ∉ env_dom Γ₂ →
-    x ∉ env_dom Γ₃ →
-    Γ₁ ⊨ e₁ : ρ : (τ + κ) ⊨ Γ₂ -∗
-    Γ₂ ⊨ e₂ : ρ : ι ⊨ Γ₃ -∗
-    (x, κ) :: Γ₂ ⊨ e₃ : ρ : ι ⊨ Γ₃ -∗
-    Γ₁ ⊨ match: e₁ with NONE => e₂ | SOME x => e₃ end : ρ : ι ⊨ Γ₃.
+  Lemma sem_typed_match_option Γ₁ Γ₂ Γ₃ e₁ x e₂ e₃ ρs κ ι: 
+    x ∉ env_dom Γ₂ → x ∉ env_dom Γ₃ →
+    Γ₁ ⊨ e₁ : ρs : Option κ ⊨ Γ₂ -∗
+    Γ₂ ⊨ e₂ : ρs : ι ⊨ Γ₃ -∗
+    (x, κ) :: Γ₂ ⊨ e₃ : ρs : ι ⊨ Γ₃ -∗
+    Γ₁ ⊨ match: e₁ with NONE => e₂ | SOME x => e₃ end : ρs : ι ⊨ Γ₃.
   Proof.
-    iIntros (??) "#He₁ #He₂ #He₃ !# %Φ %vs HΓ₁ HΦ //=".
+    iIntros (??) "#He₁ #He₂ #He₃ !# %vs HΓ₁ //=".
     iApply (ewp_bind [CaseCtx _ _]); first done.
-    iApply ("He₁" with "HΓ₁").
-    iIntros (v) "[(%w & [(-> & Hτ)|(-> & Hκ)]) HΓ₂] //="; ewp_pure_steps.
-    - iApply ("He₂" with "HΓ₂ HΦ").
+    iApply (ewp_pers_mono with "[HΓ₁]"); first (by iApply "He₁").
+    iIntros "!# %v [(%w & [(-> & _)|(-> & Hκ)]) HΓ₂] !> //="; ewp_pure_steps.
+    - iApply (ewp_pers_mono with "[HΓ₂]"); [iApply "He₂"; solve_env|eauto].
     - rewrite -subst_map_insert.
-      iApply ("He₃" with "[HΓ₂ Hκ] [HΦ]"); first solve_env.
-        iIntros (v) "[Hτι HΓ₃] //=". iApply "HΦ"; solve_env.
+      iApply (ewp_pers_mono with "[HΓ₂ Hκ]"); [iApply "He₃"; solve_env|].
+      iIntros "!# % [$ HΓ₃] //=". solve_env.
   Qed.
 
-  Lemma sem_typed_bin_op Γ₁ Γ₂ Γ₃ e₁ e₂ op τ κ ι ρ: 
+  Lemma bin_op_copy_types τ κ ι op :
+    typed_bin_op op τ κ ι → copy_ty τ ∧ copy_ty κ ∧ copy_ty ι.
+  Proof. intros []; (split; [|split]); solve_copy. Qed.
+
+  Lemma sem_typed_bin_op Γ₁ Γ₂ Γ₃ e₁ e₂ op τ κ ι ρs: 
     typed_bin_op op τ κ ι →
-    Γ₂ ⊨ e₁ : ρ : τ ⊨ Γ₃ -∗
-    Γ₁ ⊨ e₂ : ρ : κ ⊨ Γ₂ -∗
-    Γ₁ ⊨ BinOp op e₁ e₂ : ρ : ι ⊨ Γ₃.
+    Γ₂ ⊨ e₁ : ρs : τ ⊨ Γ₃ -∗
+    Γ₁ ⊨ e₂ : ρs : κ ⊨ Γ₂ -∗
+    Γ₁ ⊨ BinOp op e₁ e₂ : ρs : ι ⊨ Γ₃.
   Proof.
-    iIntros (Hop) "#He₁ #He₂ !# %Φ %vs HΓ₁ HΦ //=".
+    iIntros (Hop) "#He₁ #He₂ !# %vs HΓ₁ //=".
+    destruct (bin_op_copy_types _ _ _ _ Hop) as [Hcpyτ [Hcpyκ Hcpyι]]. 
     iApply (ewp_bind [BinOpRCtx _ _]); first done.
-    iApply ("He₂" with "HΓ₁").
-    iIntros (v) "[Hv HΓ₂] //=". 
+    iApply (ewp_pers_mono with "[HΓ₁]"); [iApply "He₂"; solve_env|eauto].
+    iIntros "!# %v [Hκ HΓ₂] //= !>". 
     iApply (ewp_bind [BinOpLCtx _ _]); first done.
-    iApply ("He₁" with "HΓ₂").
-    iIntros (w) "[Hw HΓ₃] //=". 
+    iApply (ewp_pers_mono with "[HΓ₂]"); [iApply "He₁"; solve_env|eauto].
+    rewrite Hcpyκ. iDestruct "Hκ" as "#Hκ".
+    iIntros "!# %w [Hτ HΓ₂] //= !>".
     destruct op; inversion_clear Hop;
-      iDestruct "Hv" as "(%n1 & ->)";
-      iDestruct "Hw" as "(%n2 & ->)";
-      ewp_pure_steps; try done; iApply "HΦ"; eauto.
+      iDestruct "Hτ" as "(%n1 & ->)";
+      iDestruct "Hκ" as "(%n2 & ->)";
+      ewp_pure_steps; try done; eauto.
   Qed.
   
-  Lemma sem_typed_if Γ₁ Γ₂ Γ₃ e₁ e₂ e₃ ρ τ: 
-    Γ₁ ⊨ e₁ : ρ : 𝔹 ⊨ Γ₂ -∗
-    Γ₂ ⊨ e₂ : ρ : τ ⊨ Γ₃ -∗
-    Γ₂ ⊨ e₃ : ρ : τ ⊨ Γ₃ -∗
-    Γ₁ ⊨ (if: e₁ then e₂ else e₃) : ρ : τ ⊨ Γ₃.
+  Lemma sem_typed_if Γ₁ Γ₂ Γ₃ e₁ e₂ e₃ ρs τ: 
+    Γ₁ ⊨ e₁ : ρs : 𝔹 ⊨ Γ₂ -∗
+    Γ₂ ⊨ e₂ : ρs : τ ⊨ Γ₃ -∗
+    Γ₂ ⊨ e₃ : ρs : τ ⊨ Γ₃ -∗
+    Γ₁ ⊨ (if: e₁ then e₂ else e₃) : ρs : τ ⊨ Γ₃.
   Proof.
-    iIntros "#He₁ #He₂ #He₃ !# %Φ %vs HΓ₁ HΦ //=".
+    iIntros "#He₁ #He₂ #He₃ !# %vs HΓ₁ //=".
     iApply (ewp_bind [IfCtx (subst_map vs e₂) (subst_map vs e₃)]) ;first done.
-    iApply ("He₁" with "HΓ₁").
-    iIntros (v) "((%b & ->) & HΓ₂) //=".
+    iApply (ewp_pers_mono with "[HΓ₁]"); [iApply "He₁"; solve_env|eauto].
+    iIntros "!# %v ((%b & ->) & HΓ₂) //= !>".
     destruct b; ewp_pure_steps.
-    - iApply ("He₂" with "HΓ₂"). iFrame.
-    - iApply ("He₃" with "HΓ₂"). iFrame.
+    - iApply (ewp_pers_mono with "[HΓ₂]"); [iApply "He₂"; solve_env|eauto].
+    - iApply (ewp_pers_mono with "[HΓ₂]"); [iApply "He₃"; solve_env|eauto].
   Qed.
   
   (* Type abstraction and application *)
-  Lemma sem_typed_TLam Γ₁ Γ₂ ρ e C : 
+  Lemma sem_typed_TLam Γ₁ Γ₂ ρs e C : 
     copy_env Γ₁ →
-    (∀ α, Γ₁ ⊨ e : ρ : C α ⊨ []) -∗
-    Γ₁ ++ Γ₂ ⊨ (Λ: e) : ⟨⟩ : (∀T: α , { ρ } , C α)%T ⊨ Γ₂.
+    (∀ α, Γ₁ ⊨ e : ρs : C α ⊨ []) -∗
+    Γ₁ ++ Γ₂ ⊨ (Λ: e) : ⟨⟩ : (∀T: α , ρs , C α)%T ⊨ Γ₂.
   Proof.
-    iIntros (Hcpy) "#He !# %Φ %vs HΓ₁₂ HΦ //=".
+    iIntros (Hcpy) "#He !# %vs HΓ₁₂ //=".
     iDestruct (env_sem_typed_app with "HΓ₁₂") as "[HΓ₁ HΓ₂]".
     rewrite Hcpy. iDestruct "HΓ₁" as "#HΓ₁".
-    ewp_pure_steps. iApply "HΦ". 
-    iIntros "{$HΓ₂} %α //= !#". ewp_pure_steps.
-    iApply ("He" with "HΓ₁ []"). 
-    iIntros (w) "[HC _] {$HC}".
+    ewp_pure_steps. iIntros "{$HΓ₂} %α //= !#". ewp_pure_steps.
+    iApply (ewp_pers_mono with "[HΓ₁]"); [iApply "He"; solve_env|].
+    iIntros "!# %w [$ _] //=".
   Qed.
 
-  Lemma sem_typed_TApp Γ₁ Γ₂ e ρ τ C : 
-    Γ₁ ⊨ e : ρ : (∀T: α , { ρ } , C α) ⊨ Γ₂ -∗
-    Γ₁ ⊨ e <_> : ρ : C τ ⊨ Γ₂. 
+  Lemma sem_typed_TApp Γ₁ Γ₂ e ρs τ C :
+    copy_env Γ₂ →
+    Γ₁ ⊨ e : ρs : (∀T: α , ρs , C α) ⊨ Γ₂ -∗
+    Γ₁ ⊨ e <_> : ρs : C τ ⊨ Γ₂. 
   Proof.
-    iIntros "#He !# %Φ %vs HΓ₁ HΦ /=".
+    iIntros (Hcpy) "#He !# %vs HΓ₁ /=".
     iApply (ewp_bind [AppLCtx _]); first done.
-    iApply ("He" with "HΓ₁").
-    iIntros "%w [Hw HΓ₂] //=".
-    iApply (ewp_mono with "[Hw]").
-    { iApply "Hw". }
-    iIntros (u) "HC !>". iApply "HΦ". iFrame.
+    iApply (ewp_pers_mono with "[HΓ₁]"); [iApply "He"; solve_env|].
+    iIntros "!# %w [Hw HΓ₂] //= !>".
+    iApply (ewp_pers_mono with "[Hw]"); [iApply "Hw"|].
+    rewrite {1}Hcpy. iDestruct "HΓ₂" as "#HΓ₂".
+    iIntros "!# % HC !>". iFrame "#∗".
+  Qed.
+
+  Lemma sem_typed_TApp_os Γ₁ Γ₂ (x : string) e ρ τ C :
+    x ∉ env_dom Γ₂ → 
+    Γ₁ ⊨ e : ⟨ρ,⟩ : (∀T: α , ⟨ρ,⟩ , C α) ⊨ Γ₂ -∗
+    Γ₁ ⊨ (let: x := e in x <_>) : ⟨ρ,⟩ : C τ ⊨ Γ₂. 
+  Proof.
+    iIntros (?) "#He". 
+    iApply (sem_typed_let _ Γ₂); solve_sidecond.
+    iApply sem_typed_swap_env_singl. rewrite - {3} (app_nil_r Γ₂).
+    iApply sem_typed_frame_env_os. iApply sem_typed_TApp; solve_copy.
+    iApply sem_typed_sub_nil. iApply sem_typed_var.
   Qed.
 
   (* Signature abstraction and application *)
@@ -885,129 +664,161 @@ Section compatibility.
     (∀ θ, Γ₁ ⊨ e : θ : C θ ⊨ []) -∗
     Γ₁ ++ Γ₂ ⊨ (Λ: e) : ⟨⟩ : (∀S: θ , C θ)%T ⊨ Γ₂.
   Proof.
-    iIntros "#He !# %Φ %vs HΓ₁₂ HΦ /=".
+    iIntros "#He !# %vs HΓ₁₂ /=".
     iDestruct (env_sem_typed_app with "HΓ₁₂") as "[HΓ₁ HΓ₂]".
-    ewp_pure_steps.
-    iApply "HΦ". iFrame.
-    iIntros (ρ). ewp_pure_steps.
-    iApply ("He" with "HΓ₁ []").
-    iIntros (v) "[HC _] {$HC}".
+    ewp_pure_steps. iFrame.
+    iIntros (ρs). ewp_pure_steps.
+    iApply (ewp_pers_mono with "[HΓ₁]"); [by iApply "He"|].
+    iIntros "!# % [$ _] //=".
   Qed.
 
-  Lemma sem_typed_SApp Γ₁ Γ₂ e ρ C : 
-    Γ₁ ⊨ e : ρ : (∀S: θ , C θ) ⊨ Γ₂ -∗
-    Γ₁ ⊨ e <_> : ρ : C ρ ⊨ Γ₂. 
+  Lemma sem_typed_SApp Γ₁ Γ₂ e ρs C : 
+    copy_env Γ₂ →
+    Γ₁ ⊨ e : ρs : (∀S: θ , C θ) ⊨ Γ₂ -∗
+    Γ₁ ⊨ e <_> : ρs : C ρs ⊨ Γ₂. 
   Proof.
-    iIntros "#He !# %Φ %vs HΓ₁ HΦ /=".
+    iIntros (Hcpy) "#He !# %vs HΓ₁ /=".
     iApply (ewp_bind [AppLCtx _]); first done.
-    iApply ("He" with "HΓ₁ [HΦ]").
-    iIntros (v) "[HC HΓ₂] /=".
-    iApply (ewp_mono with "HC").
-    iIntros (w) "HCρ !>". iApply "HΦ". iFrame.
+    iApply (ewp_pers_mono with "[HΓ₁]"); [by iApply "He"|].
+    iIntros "!# %v [HC HΓ₂] /= !>".
+    rewrite {1}Hcpy. iDestruct "HΓ₂" as "#HΓ₂".
+    iApply (ewp_pers_mono with "[HC]"); [iApply ("HC" $! ρs)|].
+    iIntros "!# %w HCρ !>". iFrame "∗#".
+  Qed.
+
+  Lemma sem_typed_SApp_os Γ₁ Γ₂ (x : string) e ρ C :
+    x ∉ env_dom Γ₂ → 
+    Γ₁ ⊨ e : ⟨ρ,⟩ : (∀S: θ , C θ) ⊨ Γ₂ -∗
+    Γ₁ ⊨ (let: x := e in x <_>) : ⟨ρ,⟩ : C ⟨ρ,⟩%R ⊨ Γ₂. 
+  Proof.
+    iIntros (?) "#He". 
+    iApply (sem_typed_let _ Γ₂); solve_sidecond.
+    iApply sem_typed_swap_env_singl. rewrite - {3} (app_nil_r Γ₂).
+    iApply sem_typed_frame_env_os. iApply sem_typed_SApp; solve_copy.
+    iApply sem_typed_sub_nil. iApply sem_typed_var.
   Qed.
 
   (* Existential type packing and unpacking *)
-  Lemma sem_typed_pack Γ₁ Γ₂ ρ e C τ :
-    Γ₁ ⊨ e : ρ : C τ ⊨ Γ₂ -∗
-    Γ₁ ⊨ (pack: e) : ρ : (∃: α, C α) ⊨ Γ₂. 
+  Lemma sem_typed_pack Γ₁ Γ₂ ρs e C τ :
+    Γ₁ ⊨ e : ρs : C τ ⊨ Γ₂ -∗
+    Γ₁ ⊨ (pack: e) : ρs : (∃: α, C α) ⊨ Γ₂. 
   Proof.
-    iIntros "#He %Φ %vs !# HΓ₁ HΦ //=".
+    iIntros "#He %vs !# HΓ₁ //=".
     iApply (ewp_bind [AppRCtx _]); first done.
-    iApply ("He" with "HΓ₁").
-    iIntros (v) "[Hτv HΓ₂] //=".
-    unfold exist_pack. ewp_pure_steps.
-    iApply "HΦ". iFrame. by iExists τ. 
+    iApply (ewp_pers_mono with "[HΓ₁]"); [by iApply "He"|].
+    iIntros "!# %v [Hτv HΓ₂] //= !>".
+    unfold exist_pack. ewp_pure_steps. iFrame.
+    by iExists τ. 
   Qed.
 
-  Lemma sem_typed_unpack Γ₁ Γ₂ Γ₃ x ρ e₁ e₂ κ C :
+  Lemma sem_typed_unpack Γ₁ Γ₂ Γ₃ x ρs e₁ e₂ κ C :
     x ∉ env_dom Γ₂ → x ∉ env_dom Γ₃ →
-    Γ₁ ⊨ e₁ : ρ : (∃: α, C α) ⊨ Γ₂ -∗
-    (∀ τ, (x, C τ) :: Γ₂ ⊨ e₂ : ρ : κ ⊨ Γ₃) -∗
-    Γ₁ ⊨ (unpack: x := e₁ in e₂) : ρ : κ ⊨ Γ₃.
+    Γ₁ ⊨ e₁ : ρs : (∃: α, C α) ⊨ Γ₂ -∗
+    (∀ τ, (x, C τ) :: Γ₂ ⊨ e₂ : ρs : κ ⊨ Γ₃) -∗
+    Γ₁ ⊨ (unpack: x := e₁ in e₂) : ρs : κ ⊨ Γ₃.
   Proof.
-    iIntros (??) "#He₁ #He₂ %Φ %vs !# HΓ₁ HΦ //=".
+    iIntros (??) "#He₁ #He₂ %vs !# HΓ₁ //=".
     iApply (ewp_bind [AppRCtx _]); first done.
-    iApply ("He₁" with "HΓ₁").
-    iIntros (w) "[(%τ & Hτw) HΓ₂] //=". unfold exist_unpack.
+    iApply (ewp_pers_mono with "[HΓ₁]"); [by iApply "He₁"|].
+    iIntros "!# %w [(%τ & Hτw) HΓ₂] //= !>". unfold exist_unpack.
     ewp_pure_steps. rewrite -subst_map_insert.
-    iApply ("He₂" with "[HΓ₂ Hτw]"); first solve_env.
-    iIntros (u) "[Hκ HΓ₃]". iApply "HΦ"; solve_env.
+    iApply (ewp_pers_mono with "[HΓ₂ Hτw]"); [iApply "He₂";solve_env|].
+    iIntros "!# %u [Hκ HΓ₃]". solve_env.
   Qed.
 
   (* Recursive type rules *)
-  Lemma sem_typed_fold Γ₁ Γ₂ e ρ C `{NonExpansive C}:
-    Γ₁ ⊨ e : ρ : (C (μT: α, C α)) ⊨ Γ₂ -∗
-    Γ₁ ⊨ (fold: e) : ρ : (μT: α, C α) ⊨ Γ₂.
+  Lemma sem_typed_fold Γ₁ Γ₂ e ρs C `{NonExpansive C}:
+    Γ₁ ⊨ e : ρs : (C (μT: α, C α)) ⊨ Γ₂ -∗
+    Γ₁ ⊨ (fold: e) : ρs : (μT: α, C α) ⊨ Γ₂.
   Proof.
-    iIntros "#He %Φ %vs !# HΓ₁ HΦ //=".
-    iApply (ewp_bind [AppRCtx _]); first done. 
-    iApply ("He" with "HΓ₁").
-    iIntros "%w [HC HΓ₂] //=". 
-    unfold rec_fold. ewp_pure_steps. iApply "HΦ".
+    iIntros "#He %vs !# HΓ₁ //=".
+    iApply (ewp_bind [AppRCtx _]); first done.
+    iApply (ewp_pers_mono with "[HΓ₁]"); [by iApply "He"|].
+    iIntros "!# %w [HC HΓ₂] //= !>".
+    unfold rec_fold. ewp_pure_steps. 
     iFrame. by iApply sem_ty_rec_unfold. 
   Qed.
 
-  Lemma sem_typed_unfold Γ₁ Γ₂ e ρ C `{NonExpansive C}:
-    Γ₁ ⊨ e : ρ : (μT: α, C α) ⊨ Γ₂ -∗
-    Γ₁ ⊨ (unfold: e) : ρ : (C (μT: α, C α)) ⊨ Γ₂.
+  Lemma sem_typed_unfold Γ₁ Γ₂ e ρs C `{NonExpansive C}:
+    Γ₁ ⊨ e : ρs : (μT: α, C α) ⊨ Γ₂ -∗
+    Γ₁ ⊨ (unfold: e) : ρs : (C (μT: α, C α)) ⊨ Γ₂.
   Proof.
-    iIntros "#He %Φ %vs !# HΓ₁ HΦ //=".
+    iIntros "#He %vs !# HΓ₁ //=".
     iApply (ewp_bind [AppRCtx _]); first done. 
-    iApply ("He" with "HΓ₁").
-    iIntros "%w [Hμ HΓ₂] //=". 
+    iApply (ewp_pers_mono with "[HΓ₁]"); [by iApply "He"|].
+    iIntros "!# %w [Hμ HΓ₂] //= !>". 
     rewrite sem_ty_rec_unfold. 
     unfold rec_unfold. ewp_pure_steps. 
-    iApply "HΦ". iFrame.
+    iFrame.
   Qed.
 
   (* List type rules *)
   Lemma sem_typed_nil Γ τ: 
     ⊢ Γ ⊨ NIL : ⟨⟩ : List τ ⊨ Γ.
   Proof.
-    iIntros "!# %Φ %vs HΓ HΦ //=". 
-    ewp_pure_steps. unfold sem_ty_list. iApply "HΦ".
+    iIntros "!# %vs HΓ //=". 
+    ewp_pure_steps. unfold sem_ty_list. 
     rewrite sem_ty_rec_unfold. iIntros "{$HΓ} !>".
     unfold ListF. iExists #(). by iLeft.
   Qed.
   
-  Lemma sem_typed_cons Γ₁ Γ₂ Γ₃ e₁ e₂ ρ τ: 
-    Γ₂ ⊨ e₁ : ρ : τ ⊨ Γ₃-∗
-    Γ₁ ⊨ e₂ : ρ : List τ ⊨ Γ₂-∗
-    Γ₁ ⊨ CONS e₁ e₂ : ρ : List τ ⊨ Γ₃.
+  Lemma sem_typed_cons Γ₁ Γ₂ Γ₃ e₁ e₂ ρs τ:
+    Γ₂ ⊨ e₁ : ⟨ρs.1,⟩ : τ ⊨ Γ₃-∗
+    Γ₁ ⊨ e₂ : ρs : List τ ⊨ Γ₂-∗
+    Γ₁ ⊨ CONS e₁ e₂ : ρs : List τ ⊨ Γ₃.
   Proof.
-    iIntros "#He₁ #He₂ !# %Φ %vs HΓ₁ HΦ //=". 
+    iIntros "#He₁ #He₂ !# %vs HΓ₁ //=". 
     iApply (ewp_bind [InjRCtx; PairRCtx _]); first done.
-    iApply ("He₂" with "HΓ₁").
-    iIntros (l) "[Hl HΓ₂] //=".
+    iApply (ewp_pers_mono with "[HΓ₁]"); [by iApply "He₂"|].
+    iIntros "!# %l [Hl HΓ₂] //= !>".
     iApply (ewp_bind [InjRCtx; PairLCtx _]); first done.
-    iApply ("He₁" with "HΓ₂").
-    iIntros (x) "[Hx HΓ₃] //=". ewp_pure_steps.
-    iApply "HΦ".
+    iApply ewp_ms_prot_mono; [iApply sig_le_nil|].
+    iApply (ewp_mono with "[HΓ₂]"); [by iApply "He₁"|].
+    iIntros "%x [Hx HΓ₃] //= !>". ewp_pure_steps.
     unfold sem_ty_list. rewrite !sem_ty_rec_unfold.
     iIntros "{$HΓ₃} !>". iExists (x,l)%V. iRight. iSplit; first done.
     iExists x, l. iFrame; iSplit; first done.
     by rewrite sem_ty_rec_unfold. 
   Qed.
-  
-  Lemma sem_typed_match_list Γ₁ Γ₂ Γ₃ x xs e₁ e₂ e₃ ρ τ κ :
+
+  Lemma sem_typed_cons_ms Γ₁ Γ₂ Γ₃ (x₁ x₂ : string) e₁ e₂ ρs τ:
+    x₂ ∉ env_dom Γ₂ → x₂ ∉ env_dom Γ₃ → x₁ ∉ env_dom Γ₃ → x₁ ≠ x₂ → 
+    copy_ty τ →
+    Γ₂ ⊨ e₁ : ρs : τ ⊨ Γ₃ -∗
+    Γ₁ ⊨ e₂ : ρs : List τ ⊨ Γ₂-∗
+    Γ₁ ⊨ (let: x₂ := e₂ in let: x₁ := e₁ in CONS x₁ x₂) : ρs : List τ ⊨ Γ₃.
+  Proof.
+    iIntros (???? Hcpy) "#He₁ #He₂".
+    iApply (sem_typed_let _ Γ₂); solve_sidecond.
+    iApply (sem_typed_let _ ((x₂, List τ) :: Γ₃)); solve_sidecond.
+    { iApply sem_typed_frame_ms; first by apply copy_ty_list. iApply "He₁". }
+    iApply sem_typed_sub_nil.
+    iApply (sem_typed_cons _ ((x₁, τ) :: Γ₃)); [iApply sem_typed_var|].
+    iApply sem_typed_swap_second.
+    iApply sem_typed_var.
+  Qed.
+
+  Lemma sem_typed_match_list Γ₁ Γ₂ Γ₃ x xs e₁ e₂ e₃ ρs τ κ :
     x ∉ (env_dom Γ₂) -> xs ∉ (env_dom Γ₂) ->
     x ∉ (env_dom Γ₃) -> xs ∉ (env_dom Γ₃) ->
     x ≠ xs ->
-    Γ₁ ⊨ e₁ : ρ : List τ ⊨ Γ₂ -∗
-    Γ₂ ⊨ e₂ : ρ : κ ⊨ Γ₃ -∗
-    (x, τ) :: (xs, List τ) :: Γ₂ ⊨ e₃ : ρ : κ ⊨ Γ₃ -∗
+    Γ₁ ⊨ e₁ : ρs : List τ ⊨ Γ₂ -∗
+    Γ₂ ⊨ e₂ : ρs : κ ⊨ Γ₃ -∗
+    (x, τ) :: (xs, List τ) :: Γ₂ ⊨ e₃ : ρs : κ ⊨ Γ₃ -∗
     Γ₁ ⊨ list-match: e₁ with 
             CONS x => xs => e₃ 
           | NIL => e₂
-         end : ρ : κ ⊨ Γ₃.
+         end : ρs : κ ⊨ Γ₃.
   Proof.
-    iIntros (?????) "#He₁ #He₂ #He₃ !# %Φ %vs HΓ₁ HΦ //=".
-    iApply (ewp_bind [CaseCtx _ _]); first done. 
-    iApply (sem_typed_unfold with "He₁ HΓ₁ [HΦ]"). simpl.
-    iIntros (v₁) "[Hl HΓ₂]". 
+    iIntros (?????) "#He₁ #He₂ #He₃ !# %vs HΓ₁ //=".
+    iApply (ewp_bind [CaseCtx _ _]); first done. simpl.
+    iApply (ewp_pers_mono with "[HΓ₁]");
+      [iApply (sem_typed_unfold with "He₁ HΓ₁")|].
+    iIntros "!# %v₁ [Hl HΓ₂] !>". 
     iDestruct "Hl" as "(%v' & [[-> ->]|(-> & (%w₁ & %w₂ & -> & Hτ & Hμ))])"; 
     ewp_pure_steps.
-    { iApply ("He₂" with "[$HΓ₂]"). iFrame. }
+    { iApply (ewp_pers_mono with "[HΓ₂]"); 
+        [iApply ("He₂" with "[$HΓ₂]")|eauto]. }
     rewrite lookup_delete. simpl.
     rewrite decide_False; [|by intros [_ []]].
     rewrite decide_True; last done. ewp_pure_steps.
@@ -1017,338 +828,380 @@ Section compatibility.
     rewrite subst_subst_ne; [|congruence]. rewrite delete_commute.
     rewrite -subst_map_insert -delete_insert_ne; try congruence.
     rewrite -subst_map_insert. 
-    iApply ("He₃" with "[Hμ Hτ HΓ₂]"); first solve_env.
+    iApply (ewp_pers_mono with "[Hμ Hτ HΓ₂]"); [iApply "He₃"; solve_env|].
     { rewrite env_sem_typed_insert; last done; solve_env. }
-    iIntros (u) "[Hκ HΓ₃]". iApply "HΦ". iFrame.
+    iIntros "!# %u [Hκ HΓ₃]". iFrame.
     rewrite -(env_sem_typed_insert _ _ x w₁); last done.
     by rewrite -(env_sem_typed_insert _ _ xs w₂).
   Qed.
 
   (* Reference rules *)
   
-  Lemma sem_typed_alloc Γ₁ Γ₂ e ρ τ: 
-    Γ₁ ⊨ e : ρ : τ ⊨ Γ₂ -∗
-    Γ₁ ⊨ ref e : ρ : Ref τ ⊨ Γ₂.
+  Lemma sem_typed_alloc Γ₁ Γ₂ e ρs τ: 
+    Γ₁ ⊨ e : ρs : τ ⊨ Γ₂ -∗
+    Γ₁ ⊨ ref e : ρs : Ref τ ⊨ Γ₂.
   Proof.
-    iIntros "#He !# %Φ %vs HΓ₁ HΦ //=".
+    iIntros "#He !# %vs HΓ₁ //=".
     iApply (ewp_bind [AllocCtx]); first done. simpl.
-    iApply ("He" with "HΓ₁").
-    iIntros (v) "[Hτ HΓ₂]".
-    iApply ewp_alloc. iIntros "!> %l Hl !>". iApply "HΦ"; solve_env.
+    iApply (ewp_pers_mono with "[HΓ₁]"); [by iApply "He"|].
+    iIntros "!# %v [Hτ HΓ₂] !>".
+    iApply ewp_alloc. iIntros "!> %l Hl !>". solve_env.
   Qed.
   
   Lemma sem_typed_load Γ x τ: 
     ⊢ ((x, Ref τ) :: Γ ⊨ !x : ⟨⟩ : τ ⊨ (x, Ref Moved) :: Γ).
   Proof.
-    iIntros "%Φ %vs !# //= [%v (%Hrw & (%w & -> & (%l & Hl & Hτ)) & HΓ)] HΦ".
+    iIntros "%vs !# //= [%v (%Hrw & (%w & -> & (%l & Hl & Hτ)) & HΓ)]".
     rewrite Hrw. iApply (ewp_load with "Hl").
-    iIntros "!> Hl !>". iApply "HΦ". solve_env.
+    iIntros "!> Hl !>". solve_env.
   Qed.
   
   Lemma sem_typed_load_copy Γ x τ: 
     copy_ty τ →
     ⊢ ((x, Ref τ) :: Γ ⊨ !x : ⟨⟩ : τ ⊨ (x, Ref τ) :: Γ).
   Proof.
-    iIntros (Hcpy) "%Φ %vs !# //= [%v (%Hrw & (%w & -> & (%l & Hl & Hτ)) & HΓ)] HΦ".
+    iIntros (Hcpy) "%vs !# //= [%v (%Hrw & (%w & -> & (%l & Hl & Hτ)) & HΓ)]".
     rewrite Hrw. iApply (ewp_load with "Hl").
-    rewrite Hcpy. iDestruct "Hτ" as "#Hτ".
-    iIntros "!> Hl !>". iApply "HΦ". solve_env.
+    rewrite {1}Hcpy. iDestruct "Hτ" as "#Hτ".
+    iIntros "!> Hl !>". solve_env.
   Qed.
 
-  Lemma sem_typed_store Γ₁ Γ₂ x e ρ τ κ ι: 
-    (x, Ref τ) :: Γ₁ ⊨ e : ρ : ι ⊨ (x, Ref κ) :: Γ₂ -∗
-    (x, Ref τ) :: Γ₁ ⊨ (x <- e) : ρ : () ⊨ (x, Ref ι) :: Γ₂.
+  Lemma sem_typed_store Γ₁ Γ₂ x e ρs τ κ ι: 
+    (x, Ref τ) :: Γ₁ ⊨ e : ρs : ι ⊨ (x, Ref κ) :: Γ₂ -∗
+    (x, Ref τ) :: Γ₁ ⊨ (x <- e) : ρs : () ⊨ (x, Ref ι) :: Γ₂.
   Proof.
-    iIntros "#He !# %Φ %vs //= HΓ₁' HΦ //=".
+    iIntros "#He !# %vs //= HΓ₁' //=".
     iApply (ewp_bind [StoreRCtx _]); first done. simpl.
-    iApply ("He" with "HΓ₁'").
-    iIntros (w) "[Hι [%v (%Hrw & (%l & -> & (% & Hl & Hκ)) & HΓ₂)]] /=". 
+    iApply (ewp_pers_mono with "[HΓ₁']"); [iApply "He"; solve_env|].
+    iIntros "!# %w [Hι [%v (%Hrw & (%l & -> & (% & Hl & Hκ)) & HΓ₂)]] /=". 
     rewrite Hrw. iApply (ewp_store with "Hl"). 
-    iIntros "!> Hl !>". iApply "HΦ"; solve_env. 
+    iIntros "!> !> Hl !>". solve_env. 
   Qed.
 
-  Lemma sem_typed_alloc_cpy Γ₁ Γ₂ e ρ τ: 
-    Γ₁ ⊨ e : ρ : τ ⊨ Γ₂ -∗
-    Γ₁ ⊨ ref e : ρ : Refᶜ  τ ⊨ Γ₂.
+  Lemma sem_typed_alloc_cpy Γ₁ Γ₂ e ρs τ: 
+    Γ₁ ⊨ e : ρs : τ ⊨ Γ₂ -∗
+    Γ₁ ⊨ ref e : ρs : Refᶜ  τ ⊨ Γ₂.
   Proof.
-    iIntros "#He !# %Φ %vs HΓ₁ HΦ //=".
+    iIntros "#He !# %vs HΓ₁ //=".
     iApply (ewp_bind [AllocCtx]); first done. simpl.
-    iApply ("He" with "HΓ₁").
-    iIntros (v) "[Hτ HΓ₂]".
-    iApply ewp_alloc. iIntros "!> %l Hl". 
-    iApply "HΦ". iFrame.
+    iApply (ewp_pers_mono with "[HΓ₁]"); [by iApply "He"|].
+    iIntros "!# %v [Hτ HΓ₂] !>".
+    iApply ewp_alloc. iIntros "!> %l Hl". iFrame.
     iMod (inv_alloc (tyN.@l) _
        (∃ w, l ↦ w ∗ τ w)%I with "[Hl Hτ]") as "#Hinv".
     { iExists v. by iFrame. }
     iModIntro. iExists l. by auto.
   Qed.
 
-  Lemma sem_typed_load_cpy Γ₁ Γ₂ e ρ τ: 
+  Lemma sem_typed_load_cpy Γ₁ Γ₂ e ρs τ: 
     copy_ty τ →
-    Γ₁ ⊨ e : ρ : Refᶜ τ ⊨ Γ₂ -∗
-    Γ₁ ⊨ !e : ρ : τ ⊨ Γ₂.
+    Γ₁ ⊨ e : ρs : Refᶜ τ ⊨ Γ₂ -∗
+    Γ₁ ⊨ !e : ρs : τ ⊨ Γ₂.
   Proof.
-    iIntros (Hcpy) "#He %Φ %vs !# //= HΓ₁ HΦ".
+    iIntros (Hcpy) "#He %vs !# //= HΓ₁".
     iApply (ewp_bind [LoadCtx]); first done.
-    iApply ("He" with "HΓ₁").
-    iIntros (v) "[(%l & -> & Hinv) HΓ₂] /=".
+    iApply (ewp_pers_mono with "[HΓ₁]"); [by iApply "He"|].
+    iIntros "!# %v [(%l & -> & Hinv) HΓ₂] /= !>".
     iApply (ewp_atomic _ (⊤ ∖ ↑tyN.@l)).
     iMod (inv_acc _ (tyN.@l) with "Hinv") as "[(%u & >Hl & Hτ) Hclose]"; first done.
     iModIntro. iApply (ewp_load with "Hl").
     iIntros "!> Hl !>". 
-    rewrite Hcpy. iDestruct "Hτ" as "#Hτ".
+    rewrite {1}Hcpy. iDestruct "Hτ" as "#Hτ".
     iMod ("Hclose" with "[Hl]"); solve_env.
-    iModIntro. iApply "HΦ". iFrame "∗#".
   Qed.
 
-  Lemma sem_typed_store_cpy Γ₁ Γ₂ Γ₃ e₁ e₂ ρ τ: 
+  Lemma sem_typed_store_cpy Γ₁ Γ₂ Γ₃ e₁ e₂ ρs τ: 
     copy_ty τ →
-    Γ₂ ⊨ e₁ : ρ : Refᶜ τ ⊨ Γ₃ -∗
-    Γ₁ ⊨ e₂ : ρ : τ ⊨ Γ₂ -∗
-    Γ₁ ⊨ (e₁ <- e₂) : ρ : () ⊨ Γ₃.
+    Γ₂ ⊨ e₁ : ρs : Refᶜ τ ⊨ Γ₃ -∗
+    Γ₁ ⊨ e₂ : ρs : τ ⊨ Γ₂ -∗
+    Γ₁ ⊨ (e₁ <- e₂) : ρs : () ⊨ Γ₃.
   Proof.
-    iIntros (Hcpy) "#He₁ #He₂ %Φ %vs !# /= HΓ₁ HΦ /=".
+    iIntros (Hcpy) "#He₁ #He₂ %vs !# /= HΓ₁ /=".
     iApply (ewp_bind [StoreRCtx _]); first done. simpl.
-    iApply ("He₂" with "HΓ₁").
-    iIntros (w) "[Hτ HΓ₂]". 
+    iApply (ewp_pers_mono with "[HΓ₁]"); [by iApply "He₂"|].
+    iIntros "!# %w [Hτ HΓ₂] !>". 
     iApply (ewp_bind [StoreLCtx _]); first done. simpl.
-    iApply ("He₁" with "HΓ₂").
-    iIntros (u) "[(%l & -> & Hinv) HΓ₃]".
+    rewrite Hcpy. iDestruct "Hτ" as "#Hτ".
+    iApply (ewp_pers_mono with "[HΓ₂]"); [by iApply "He₁"|].
+    iIntros "!# %u [(%l & -> & Hinv) HΓ₃] !>".
     iApply (ewp_atomic _ (⊤ ∖ ↑tyN.@l)).
-    iMod (inv_acc _ (tyN.@l) with "Hinv") as "[(%u & >Hl & Hu) Hclose]"; first done.
+    iMod (inv_acc _ (tyN.@l) with "Hinv") as "[(%u & >Hl & _) Hclose]"; first done.
     iModIntro. iApply (ewp_store with "Hl"). 
     iIntros "!> Hl !>".  
-    rewrite Hcpy. iDestruct "Hτ" as "#Hτ".
     iMod ("Hclose" with "[Hl Hτ]"); solve_env.
-    iIntros "!>". iApply "HΦ"; solve_env.
   Qed.
 
-  Lemma sem_typed_replace_cpy Γ₁ Γ₂ Γ₃ e₁ e₂ ρ τ: 
-    Γ₂ ⊨ e₁ : ρ : Refᶜ τ ⊨ Γ₃ -∗
-    Γ₁ ⊨ e₂ : ρ : τ ⊨ Γ₂ -∗
-    Γ₁ ⊨ (e₁ <!- e₂) : ρ : τ ⊨ Γ₃.
+  Lemma sem_typed_replace_cpy Γ₁ Γ₂ Γ₃ e₁ e₂ ρs τ: 
+    Γ₂ ⊨ e₁ : ⟨ρs.1,⟩ : Refᶜ τ ⊨ Γ₃ -∗
+    Γ₁ ⊨ e₂ : ρs : τ ⊨ Γ₂ -∗
+    Γ₁ ⊨ (e₁ <!- e₂) : ρs : τ ⊨ Γ₃.
   Proof.
-    iIntros "#He₁ #He₂ %Φ %vs !# /= HΓ₁ HΦ /=".
+    iIntros "#He₁ #He₂ %vs !# /= HΓ₁ /=".
     iApply (ewp_bind [ReplaceRCtx _]); first done. simpl.
-    iApply ("He₂" with "HΓ₁").
-    iIntros (w) "[Hτ HΓ₂]". 
+    iApply (ewp_pers_mono with "[HΓ₁]"); [by iApply "He₂"|].
+    iIntros "!# %w [Hτ HΓ₂] !>". 
     iApply (ewp_bind [ReplaceLCtx _]); first done. simpl.
-    iApply ("He₁" with "HΓ₂").
-    iIntros (u) "[(%l & -> & Hinv) HΓ₃]".
+    iApply ewp_ms_prot_mono; [iApply sig_le_nil|].
+    iApply (ewp_mono with "[HΓ₂]"); [by iApply "He₁"|].
+    iIntros "%u [(%l & -> & Hinv) HΓ₃] !>".
     iApply (ewp_atomic _ (⊤ ∖ ↑tyN.@l)).
     iMod (inv_acc _ (tyN.@l) with "Hinv") as "[(%u & >Hl & Hu) Hclose]"; first done.
     iModIntro. iApply (ewp_replace with "Hl"). 
     iIntros "!> Hl !>".  
     iMod ("Hclose" with "[Hl Hτ]").
     { iExists w. iFrame. } 
-    iIntros "!>". iApply "HΦ"; solve_env.
+    iIntros "!>". iFrame.
   Qed.
   
   (* Effect handling rules *)
   
-  Lemma sem_typed_perform Γ₁ Γ₂ e τ (A B : sem_ty Σ → sem_sig Σ → sem_ty Σ) 
+  Lemma sem_typed_perform_os Γ₁ Γ₂ e τ ρ' (A B : sem_ty Σ → sem_sig Σ → sem_ty Σ) 
     `{ NonExpansive2 A, NonExpansive2 B } :
     let ρ := (∀μTS: θ, α, A α θ ⇒ B α θ)%R in
-    Γ₁ ⊨ e : ρ : A τ ρ ⊨ Γ₂ -∗
-    Γ₁ ⊨ (perform: e) : ρ : B τ ρ ⊨ Γ₂.
+    Γ₁ ⊨ e : ⟨ρ, ρ'⟩ : A τ ρ ⊨ Γ₂ -∗
+    Γ₁ ⊨ (perform: e) : ⟨ρ, ρ'⟩ : B τ ρ ⊨ Γ₂.
   Proof.
-    iIntros (ρ) "#He !# %Φ %vs HΓ₁ HΦ //=". rewrite /rec_perform.
-    iApply (ewp_bind [AppRCtx _; DoCtx OS]); first done.
-    iApply ("He" with "HΓ₁").
-    iIntros (v) "[Hι HΓ₂] //=".
-    iApply (ewp_bind [AppRCtx _]); first done.
+    iIntros (ρ) "#He !# %vs HΓ₁ //=". rewrite /rec_perform.
+    iApply (ewp_bind [AppRCtx _; DoCtx OS; InjLCtx]); first done.
+    iApply (ewp_pers_mono with "[HΓ₁]"); [by iApply "He"|].
+    iIntros "!# %v [Hι HΓ₂] //= !>". ewp_pure_steps.
     iApply ewp_do_os. rewrite upcl_sem_sig_rec_eff /=.
     iExists τ, v. iFrame. iSplitR; first done.
-    iIntros (b) "Hκ". ewp_pure_steps. iApply "HΦ". iFrame.
+    iIntros (b) "Hκ". ewp_pure_steps. iFrame.
   Qed.
 
-  (* Limitation: 
-     In the typing rule for the effect branch, the continuation
-     has the additional information that when called it returns
-     a value of type τ' and that env_sem_typed Γ₂ vs holds.
-     But because the type signature of the handler is simply:
-     ι ⊸ (k -{ ρ }-∘ τ' -{ ρ }-∘ τ 
-     this extra env_sem_typed Γ₂ vs is ignored and cannot be
-     used inside the handler, so we have some loss of information.
-   *)
-  Lemma sem_typed_shallow_try Γ₁ Γ₂ Γ₃ Γ' w k e h r A B τ τ' ρ' `{NonExpansive2 A, NonExpansive2 B}:
+  Lemma sem_typed_perform_ms Γ₁ Γ₂ e τ ρ (A B : sem_ty Σ → sem_sig Σ → sem_ty Σ) 
+    `{ NonExpansive2 A, NonExpansive2 B } :
+    copy_env Γ₂ →
+    let ρ' := (∀μTSₘ: θ, α, A α θ ⇒ B α θ)%R in
+    Γ₁ ⊨ e : ⟨ρ, ρ'⟩ : A τ ρ' ⊨ Γ₂ -∗
+    Γ₁ ⊨ (performₘ: e) : ⟨ρ, ρ'⟩ : B τ ρ' ⊨ Γ₂.
+  Proof.
+    iIntros (Hcpy ρ') "#He !# %vs HΓ₁ //=". rewrite /rec_perform.
+    iApply (ewp_bind [AppRCtx _; DoCtx MS; InjRCtx]); first done.
+    iApply (ewp_pers_mono with "[HΓ₁]"); [by iApply "He"|].
+    iIntros "!# %v [Hι HΓ₂] //= !>". ewp_pure_steps.
+    iApply ewp_do_ms. rewrite upcl_sem_sig_rec_eff /=.
+    iExists τ, v. iFrame. iSplitR; first done.
+    rewrite {1}Hcpy. iDestruct "HΓ₂" as "#HΓ₂".
+    iIntros "!# %b Hκ". ewp_pure_steps. iFrame "∗#".
+  Qed.
+
+  Lemma sem_typed_shallow_try Γ₁ Γ₂ Γ₃ Γ' w k e hos hms r A₁ B₁ A₂ B₂ τ τ' ρs 
+        `{NonExpansive2 A₁, NonExpansive2 B₁, NonExpansive2 A₂, NonExpansive2 B₂}:
     w ∉ env_dom Γ₂ → w ∉ env_dom Γ' → k ∉ env_dom Γ' →
     w ∉ env_dom Γ₃ → k ∉ env_dom Γ₃ → w ≠ k →
-    let ρ := (∀μTS: θ, α, A α θ  ⇒ B α θ)%R in
-    Γ₁ ⊨ e : ρ : τ' ⊨ Γ₂ -∗
-    (∀ α, (w, A α ρ) :: (k, B α ρ -{ ρ }-∘ τ') :: Γ' ⊨ h : ρ' : τ ⊨ Γ₃) -∗
-    (w, τ') :: Γ₂ ++ Γ' ⊨ r : ρ' : τ ⊨ Γ₃ -∗
-    Γ₁ ++ Γ' ⊨ (shallow-try: e with effect (λ: w k, h) | return (λ: w, r) end) : ρ' : τ ⊨ Γ₃.
+    let ρ₁ := (∀μTS: θ, α, A₁ α θ ⇒ B₁ α θ)%R in
+    let ρ₂ := (∀μTSₘ: θ, α, A₂ α θ ⇒ B₂ α θ)%R in
+    Γ₁ ⊨ e : ⟨ρ₁, ρ₂⟩ : τ' ⊨ Γ₂ -∗
+    (∀ α, (w, A₁ α ρ₁) :: (k, B₁ α ρ₁ -{ ⟨ρ₁, ρ₂⟩ }-∘ τ') :: Γ' ⊨ hos : ρs : τ ⊨ Γ₃) -∗
+    (∀ α, (w, A₂ α ρ₂) :: (k, B₂ α ρ₂ -{ ⟨ρ₁, ρ₂⟩ }-> τ') :: Γ' ⊨ hms : ρs : τ ⊨ Γ₃) -∗
+    (w, τ') :: Γ₂ ++ Γ' ⊨ r : ρs : τ ⊨ Γ₃ -∗
+    Γ₁ ++ Γ' ⊨ (shallow-try-dual: e
+                  effect  (λ: w k, hos) 
+                | effectₘ (λ: w k, hms) 
+                | return  (λ: w, r) end) : ρs : τ ⊨ Γ₃.
   Proof.
-    iIntros (??????) "%ρ #He #Hh #Hr !# %Φ %vs HΓ₁' HΦ //=".
-    iDestruct (env_sem_typed_app with "HΓ₁'") as "[HΓ₁ HΓ']".
-    ewp_pure_steps.
-    iApply (ewp_try_with _ _ _ (λ v, τ' v ∗ env_sem_typed Γ₂ vs) 
-                    with "[HΓ₁] [HΓ' HΦ]"). 
-    { iApply ("He" with "HΓ₁"). iIntros "* [Hτ' HΓ₂] {$Hτ' $HΓ₂}". }
-    iSplit; [|iSplit; iIntros (v c)];
-    last (iIntros "?"; by rewrite upcl_bottom).
+    iIntros (??????) "%ρ₁ %ρ₂ #He #Hhos #Hhms #Hr !# %vs HΓ₁Γ' //=".
+    iDestruct (env_sem_typed_app with "HΓ₁Γ'") as "[HΓ₁ HΓ']".
+    iApply (ewp_try_with _ _ _ (λ v, τ' v ∗ ⟦ Γ₂ ⟧ vs)%I with "[HΓ₁] [HΓ']"). 
+    { iApply (ewp_pers_mono with "[HΓ₁]"); [by iApply "He"|eauto]. }
+    iSplit; [|iSplit; iIntros (v c)].
     - iIntros (v) "[Hv HΓ₂] //=". ewp_pure_steps.
       rewrite -subst_map_insert.
-      iApply ("Hr" with "[HΓ₂ HΓ' Hv]"). 
-      { iExists v. rewrite env_sem_typed_app. solve_env. }
-      + iIntros (u) "[Hw HΓ₃] //=". iApply "HΦ". solve_env.
+      iApply (ewp_pers_mono with "[HΓ₂ HΓ' Hv]"); [iApply "Hr"|].
+      { iExists v. rewrite env_sem_typed_app; solve_env. }
+      iIntros "!# % [Hτ HΓ₃]"; solve_env.
     - rewrite upcl_sem_sig_rec_eff.
-      iIntros "(%α & %a & -> & Ha & Hκb) //=". ewp_pure_steps.
+      iIntros "(%α & %a & <- & Ha & Hκb) //=". rewrite /select_on_sum. ewp_pure_steps.
       rewrite decide_True; [|split; first done; by injection].
       rewrite subst_subst_ne; last done.
       rewrite -subst_map_insert -delete_insert_ne; last done.
       rewrite -subst_map_insert.
-      iApply ("Hh" with "[HΓ' Hκb Ha]"); first solve_env.
-      + iSplitR "HΓ'"; [|by (do 2 (rewrite -env_sem_typed_insert; try done))].
-        iIntros (b ws) "_ Hκ". rewrite env_dom_nil /=. 
-        iApply (ewp_mono with "[Hκ Hκb]"); [by iApply "Hκb"|].
-        iIntros (?) "[Hτ' _] !> //=". iFrame.
-      + iIntros (u) "[Hu HΓ₃]". iApply "HΦ". iFrame.
-        rewrite -(env_sem_typed_insert _ _ w v); last done.
+      iApply (ewp_pers_mono with "[HΓ' Hκb Ha]"); [iApply "Hhos"; solve_env; iSplitR "HΓ'"|].
+      + iIntros (b) "Hκ /=".
+        iApply (ewp_pers_mono with "[Hκ Hκb]"); [by iApply "Hκb"|].
+        iIntros "!# % [Hτ' _] !> //=".
+      + by (do 2 (rewrite -env_sem_typed_insert; try done)).
+      + iIntros "!# %u [$ HΓ₃] !>".
+        rewrite -(env_sem_typed_insert _ _ w a); last done.
+        by rewrite -(env_sem_typed_insert _ _ k c).
+    - rewrite upcl_sem_sig_rec_eff.
+      iIntros "(%α & %a & <- & Ha & Hκb) //=". rewrite /select_on_sum. ewp_pure_steps.
+      rewrite decide_True; [|split; first done; by injection].
+      rewrite subst_subst_ne; last done.
+      rewrite -subst_map_insert -delete_insert_ne; last done.
+      rewrite -subst_map_insert.
+      iApply (ewp_pers_mono with "[HΓ' Hκb Ha]"); [iApply "Hhms"; solve_env|].
+      + iDestruct "Hκb" as "#Hκb".
+        iIntros "!# %b Hκ /=".
+        iApply (ewp_pers_mono with "[Hκ]"); [by iApply "Hκb"|].
+        iIntros "!# % [Hτ' _] !> //=".
+      + by (do 2 (rewrite -env_sem_typed_insert; try done)).
+      + iIntros "!# %u [$ HΓ₃] !>".
+        rewrite -(env_sem_typed_insert _ _ w a); last done.
         by rewrite -(env_sem_typed_insert _ _ k c).
   Qed.
   
-  Lemma sem_typed_deep_try Γ₁ Γ' Γ₂ Γ₃ e w k h r ρ' A B τ τ' `{NonExpansive2 A, NonExpansive2 B}:
-    w ∉ env_dom Γ₂ → w ∉ env_dom Γ' → w ∉ env_dom Γ₃ →
-    k ∉ env_dom Γ' → k ∉ env_dom Γ₃ → w ≠ k → copy_env Γ' →
-    let ρ := (∀μTS: θ , α, A α θ ⇒ B α θ)%R in
-    Γ₁ ⊨ e : ρ : τ ⊨ Γ₂ -∗
-    (∀ α, (w, A α ρ) :: (k, B α ρ -{ ρ' }-∘ τ') :: Γ' ⊨ h : ρ' : τ' ⊨ Γ₃) -∗
-    (w, τ) :: Γ₂ ++ Γ' ⊨ r : ρ' : τ' ⊨ Γ₃ -∗
-    Γ₁ ++ Γ' ⊨ (deep-try: e with effect (λ: w k, h) | return (λ: w, r) end) : ρ' : τ' ⊨ Γ₃.
+  Lemma sem_typed_shallow_try_os Γ₁ Γ₂ Γ₃ Γ' w k e h r A B τ τ' ρs `{NonExpansive2 A, NonExpansive2 B }:
+    w ∉ env_dom Γ₂ → w ∉ env_dom Γ' → k ∉ env_dom Γ' →
+    w ∉ env_dom Γ₃ → k ∉ env_dom Γ₃ → w ≠ k →
+    let ρ := (∀μTS: θ, α, A α θ ⇒ B α θ)%R in
+    Γ₁ ⊨ e : ⟨ρ,⟩ : τ' ⊨ Γ₂ -∗
+    (∀ α, (w, A α ρ) :: (k, B α ρ -{ ⟨ρ, ∀μTSₘ: θ, α, ⊥ ⇒ ⊥⟩ }-∘ τ') :: Γ' ⊨ h : ρs : τ ⊨ Γ₃) -∗
+    (w, τ') :: Γ₂ ++ Γ' ⊨ r : ρs : τ ⊨ Γ₃ -∗
+    Γ₁ ++ Γ' ⊨ (shallow-try-dual: e
+                  effect  (λ: w k, h) 
+                | effectₘ (λ: w k, w) 
+                | return  (λ: w, r) end) : ρs : τ ⊨ Γ₃.
   Proof.
-    iIntros (?????? Hcpy) "%ρ #He #Hh #Hr !# %Φ %vs HΓ₁' HΦ //=".
-    iDestruct (env_sem_typed_app with "HΓ₁'") as "[HΓ₁ HΓ']".
+    iIntros (??????) "%ρ #He #Hh #Hr".
+    set Bot := (λ (_ : sem_ty Σ) (_ : sem_sig Σ), @sem_ty_void Σ).
+    iApply (sem_typed_shallow_try _ Γ₂ _ _ _ _ _ _ _ _ A B Bot Bot with "[] [Hh] [] [Hr]"); try assumption.
+    - iApply sem_typed_sub_sig; [|iApply "He"]. rewrite /ρ.
+      apply sigs_le_comp; [apply sig_le_refl|apply sig_le_nil].
+    - simpl. rewrite /ρ. iIntros (α). iApply ("Hh" $! α).
+    - iIntros (α). rewrite /Bot /=. 
+      iApply sem_typed_sub_nil. iApply sem_typed_bot_in_env.
+    - iApply "Hr".
+  Qed.
+
+  Lemma sem_typed_shallow_try_ms Γ₁ Γ₂ Γ₃ Γ' w k e h r A B τ τ' ρs `{NonExpansive2 A, NonExpansive2 B }:
+    w ∉ env_dom Γ₂ → w ∉ env_dom Γ' → k ∉ env_dom Γ' →
+    w ∉ env_dom Γ₃ → k ∉ env_dom Γ₃ → w ≠ k →
+    let ρ := (∀μTSₘ: θ, α, A α θ ⇒ B α θ)%R in
+    Γ₁ ⊨ e : ⟨,ρ⟩ : τ' ⊨ Γ₂ -∗
+    (∀ α, (w, A α ρ) :: (k, B α ρ -{ ⟨∀μTS: θ, α, ⊥ ⇒ ⊥, ρ⟩ }-> τ') :: Γ' ⊨ h : ρs : τ ⊨ Γ₃) -∗
+    (w, τ') :: Γ₂ ++ Γ' ⊨ r : ρs : τ ⊨ Γ₃ -∗
+    Γ₁ ++ Γ' ⊨ (shallow-try-dual: e
+                  effect  (λ: w k, w) 
+                | effectₘ (λ: w k, h) 
+                | return  (λ: w, r) end) : ρs : τ ⊨ Γ₃.
+  Proof.
+    iIntros (??????) "%ρ #He #Hh #Hr".
+    set Bot := (λ (_ : sem_ty Σ) (_ : sem_sig Σ), @sem_ty_void Σ).
+    iApply (sem_typed_shallow_try _ Γ₂ _ _ _ _ _ _ _ _ Bot Bot A B with "[] [Hh] [] [Hr]"); try assumption.
+    - iApply sem_typed_sub_sig; [|iApply "He"]. rewrite /ρ.
+      apply sigs_le_comp; [apply sig_le_nil|apply sig_le_refl].
+    - iIntros (α). rewrite /Bot /=. 
+      iApply sem_typed_sub_nil. iApply sem_typed_bot_in_env.
+    - simpl. rewrite /ρ. iIntros (α). iApply ("Hh" $! α).
+    - iApply "Hr".
+  Qed.
+
+  Lemma sem_typed_deep_try Γ₁ Γ₂ Γ₃ Γ' w k e hos hms r A₁ B₁ A₂ B₂ τ τ' ρs 
+        `{NonExpansive2 A₁, NonExpansive2 B₁, NonExpansive2 A₂, NonExpansive2 B₂}:
+    w ∉ env_dom Γ₂ → w ∉ env_dom Γ' → k ∉ env_dom Γ' →
+    w ∉ env_dom Γ₃ → k ∉ env_dom Γ₃ → w ≠ k → copy_env Γ' →
+    let ρ₁ := (∀μTS: θ, α, A₁ α θ ⇒ B₁ α θ)%R in
+    let ρ₂ := (∀μTSₘ: θ, α, A₂ α θ ⇒ B₂ α θ)%R in
+    Γ₁ ⊨ e : ⟨ρ₁, ρ₂⟩ : τ' ⊨ Γ₂ -∗
+    (∀ α, (w, A₁ α ρ₁) :: (k, B₁ α ρ₁ -{ ρs }-∘ τ) :: Γ' ⊨ hos : ρs : τ ⊨ Γ₃) -∗
+    (∀ α, (w, A₂ α ρ₂) :: (k, B₂ α ρ₂ -{ ρs }-> τ) :: Γ' ⊨ hms : ρs : τ ⊨ Γ₃) -∗
+    (w, τ') :: Γ₂ ++ Γ' ⊨ r : ρs : τ ⊨ Γ₃ -∗
+    Γ₁ ++ Γ' ⊨ (deep-try-dual: e
+                  effect  (λ: w k, hos) 
+                | effectₘ (λ: w k, hms) 
+                | return  (λ: w, r) end) : ρs : τ ⊨ Γ₃.
+  Proof.
+    iIntros (?????? Hcpy) "%ρ₁ %ρ₂ #He #Hhos #Hhms #Hr !# %vs HΓ₁Γ' //=".
+    iDestruct (env_sem_typed_app with "HΓ₁Γ'") as "[HΓ₁ HΓ']".
     rewrite Hcpy. iDestruct "HΓ'" as "#HΓ'".
-    ewp_pure_steps. iApply (ewp_mono with "[HΓ₁] [HΦ]").
-    2: { simpl. iIntros "* H !>". iApply "HΦ". iApply "H". }
-    iApply (ewp_deep_try_with _ _ _ (λ v, τ v ∗ env_sem_typed Γ₂ vs) 
-                         with "[HΓ₁] []").
-    { iApply ("He" with "HΓ₁"). iIntros "* H {$H}". }
-    iLöb as "IH". rewrite !deep_handler_unfold.
-    iSplit; [|iSplit; iIntros (v c)];
-    last (iIntros "?"; by rewrite upcl_bottom).
+    rewrite /select_on_sum. ewp_pure_steps. 
+    iApply (ewp_deep_try_with _ _ _ (λ v, τ' v ∗ env_sem_typed Γ₂ vs) with "[HΓ₁] []").
+    { iApply (ewp_pers_mono with "[HΓ₁]"); [by iApply "He"|eauto]. }
+    iLöb as "IH". rewrite {2}deep_handler_unfold.
+    iSplit; [|iSplit; iIntros (v c)].
     - iIntros (v) "[Hv HΓ₂] //=". ewp_pure_steps.
-      rewrite -subst_map_insert. 
-      iApply ("Hr" with "[Hv HΓ₂ HΓ']").
-      { iExists v. rewrite env_sem_typed_app. solve_env. }
-      + iIntros (?) "[Hτ' HΓ₃] {$Hτ'}"; solve_env.
+      rewrite -subst_map_insert.
+      iApply (ewp_pers_mono with "[HΓ₂ HΓ' Hv]"); [iApply "Hr"|].
+      { iExists v. rewrite env_sem_typed_app; solve_env. }
+      iIntros "!# % [Hτ HΓ₃]"; solve_env.
     - rewrite upcl_sem_sig_rec_eff.
-      iIntros "(%α & %a & -> & Ha & Hκb)". ewp_pure_steps.
+      iIntros "(%α & %a & <- & Ha & Hκb) //=". ewp_pure_steps.
       rewrite decide_True; [|split; first done; by injection].
       rewrite subst_subst_ne; last done.
       rewrite -subst_map_insert -delete_insert_ne; last done.
       rewrite -subst_map_insert.
-      iApply ("Hh" with "[Ha HΓ' Hκb]").
-      + solve_env. 
-        iSplitL "Hκb"; [|by (do 2 (rewrite -env_sem_typed_insert; try done))].
-        iIntros (b ws) "_ Hb". iApply (ewp_mono with "[Hb Hκb] []").
-        { iApply ("Hκb" with "Hb []"). rewrite !deep_handler_unfold. iApply "IH". }
-        iIntros "* [Hτ' _] !> {$Hτ'}". 
-      + iIntros (u) "[Hτ' HΓ₃] {$Hτ'}".
-        rewrite -(env_sem_typed_insert _ _ w v); last done.
+      iApply (ewp_pers_mono with "[HΓ' Hκb Ha]"); [iApply "Hhos"; solve_env; iSplitR "HΓ'"|].
+      + iIntros (b) "Hκ /=".
+        iApply (ewp_pers_mono with "[Hκ Hκb]"); [iApply ("Hκb" with "Hκ IH")|].
+        iIntros "!# % [Hτ' _] !> //=".
+      + by (do 2 (rewrite -env_sem_typed_insert; try done)).
+      + iIntros "!# %u [$ HΓ₃] !>".
+        rewrite -(env_sem_typed_insert _ _ w a); last done.
         by rewrite -(env_sem_typed_insert _ _ k c).
-    Qed.
-
-  Lemma sem_typed_deep_try_alt Γ₁ Δ Γ₂ Γ₃ e w k h r ρ' A B τ τ' `{NonExpansive2 A, NonExpansive2 B}:
-    w ∉ env_dom Γ₂ → w ∉ env_dom Δ → w ∉ env_dom Γ₃ →
-    k ∉ env_dom Δ → k ∉ env_dom Γ₃ → w ≠ k →
-    env_dom Γ₃ ⊆ env_dom Δ →
-    let ρ := (∀μTS: θ, α, A α θ ⇒ B α θ)%R in
-    Γ₁ ⊨ e : ρ : τ ⊨ Γ₂ -∗
-    (∀ α, [(w, A α ρ) ; (k, B α ρ -{ ρ' ; Δ ; Γ₃ }-∘ τ')] ⊨ h : ρ' : (() -{ ρ' ; Δ ; Γ₃ }-∘ τ') ⊨ []) -∗
-    (w, τ) :: Γ₂ ⊨ r : ρ' : (() -{ ρ' ; Δ ; Γ₃ }-∘ τ') ⊨ [] -∗
-    Γ₁ ++ Δ ⊨ (deep-try-alt: e  thread (env_dom Δ) with  
-                                effect k => w => h 
-                              | return w => r end) : ρ' : τ' ⊨ Γ₃. 
-  Proof.
-    iIntros (???????) "%ρ #He #Hh #Hr %Φ !# %vs HΓ₁Δ HΦ /=".
-    iDestruct (env_sem_typed_app with "HΓ₁Δ") as "[HΓ₁ HΔ]".
-    rewrite subst_map_app_mult.
-    iDestruct (subst_map_var with "HΔ") as "[%ws %Hrw]". 
-    rewrite map_map app_mult_cons.
-    replace (λ x: string, subst_map vs x) with (subst_map vs ∘ Var) by done.
-    rewrite Hrw. 
-    assert (Hcons : ∀ xs, map Val xs ++ [ Val #() ] = map Val (xs ++ [ #() ])).
-    { intros xs. induction xs; first done. simpl. by rewrite IHxs. }
-    rewrite Hcons. iApply ewp_bind_app_mult.
-    iApply (ewp_mono _ _ (λ v, (() -{ ρ'; Δ; Γ₃ }-∘ τ') v) with "[HΓ₁] [HΔ HΦ]").
-    2: { iIntros "% Hv !>". rewrite -Hcons -Hrw -app_mult_cons.
-         iApply (ewp_mono with "[Hv HΔ]"); [by iApply ("Hv" with "HΔ")|].
-         iIntros (?) "[Hτ' HΓ₃] !>". iApply "HΦ". iFrame. }
-    iSimpl. ewp_pure_steps. 
-    iApply (ewp_deep_try_with _ _ _ (λ v, τ v ∗ env_sem_typed Γ₂ vs) with "[HΓ₁] []").
-    { iApply ("He" with "HΓ₁"). iIntros "* H {$H}". }
-    iLöb as "IH". rewrite {2}deep_handler_unfold.
-    iSplit; [|iSplit; iIntros (v c)];
-    last (iIntros "?"; by rewrite upcl_bottom).
-    - iIntros (v) "[Hτ HΓ₂] //=". ewp_pure_steps.
-      rewrite -subst_map_insert. 
-      iApply ("Hr" with "[Hτ HΓ₂]"); first solve_env.
-      iIntros (?) "[$ _] /=".
     - rewrite upcl_sem_sig_rec_eff.
-      iIntros "(%α & %a & -> & Ha & Hκb)". ewp_pure_steps. 
-      do 2 (rewrite decide_True; [|split; first done; by injection]). iSimpl.
-      rewrite !/lambdas_norm lookup_delete.
-      rewrite decide_False; last tauto. iSimpl.
-      rewrite decide_False; last done. iSimpl.
-      rewrite decide_True; last done. ewp_pure_steps.
-      rewrite delete_idemp delete_commute -subst_map_insert -delete_insert_ne; last done.
-      rewrite -subst_map_singleton !subst_map_ctx_lambda delete_list_singleton_ne; last done.
-      iSimpl. rewrite delete_singleton_ne; last done. rewrite subst_map_app_mult. iSimpl.
-      rewrite lookup_insert lookup_singleton_ne; last done. rewrite map_map. 
-      replace (map (λ x: string, subst_map {[k := c]} x) (env_dom Δ)) with
-              (map Var (env_dom Δ)).
-      2: { clear - k c Δ H2. induction Δ as [|[] ]; first done. rewrite env_dom_cons /=.
-           rewrite env_dom_cons in H2. edestruct (not_elem_of_cons (env_dom Δ)) as [[] _]; first done.
-           rewrite lookup_singleton_ne; last done. by rewrite IHΔ. }
-      destruct Δ as [|[x κ'] Δ'] eqn:HΔeq.
-      + rewrite !env_dom_nil. iSimpl. ewp_pure_steps. 
-        replace Γ₃ with ([] : env Σ) by 
-          (symmetry; apply (map_eq_nil fst); by apply list_nil_subseteq). 
-        rewrite -subst_map_insert.
-        iApply ("Hh" with "[Ha Hκb]"); 
-          last (iIntros (?) "[Hτ' _]"; ewp_pure_steps; iFrame; iIntros "_"; ewp_pure_steps; iFrame).
-        solve_env. iIntros (u us) "_ Hκ". rewrite env_dom_nil /=. ewp_pure_steps.
-        rewrite decide_True; last done.
-        iApply (ewp_bind [AppLCtx _]); first done.
-        iApply (ewp_mono with "[Hκ Hκb]"); [iApply ("Hκb" with "Hκ")|].
-        { iNext. rewrite delete_commute. by iApply "IH". }
-        iIntros (?) "H !> /=". by iApply "H".
-      + rewrite {5}env_dom_cons. iSimpl. ewp_pure_steps.
-        rewrite -subst_map_insert.
-        iApply ("Hh" with "[Ha Hκb]"); [|iIntros (u) "[$ _]"].
-        iExists v. iFrame. iSplit.
-        { iPureIntro. rewrite insert_commute; last done. apply lookup_insert. }
-        set k' := (λλ*λ: x, env_dom Δ', w, ((c w) <_ map Var (env_dom ((x, κ')%core :: Δ')) _>) #())%V.
-        iExists k'. iSplit; [iPureIntro; apply lookup_insert|].
-        iSplitL "Hκb"; last done.
-        iIntros (u us) "HΔ Hκ". rewrite /k'.
-        iApply (ewp_bind [AppLCtx _]); first done.
-        iApply (ewp_app_mult with "HΔ"). iIntros "HΔ". iSimpl.
-        ewp_pure_steps. rewrite -subst_map_insert -HΔeq subst_map_app_mult. iSimpl.
-        rewrite lookup_insert. 
-        set uus := (<[w:=u]> (us ∖ delete (env_dom Δ) us)).
-        rewrite map_map. replace (λ x0 : string, (subst_map uus x0)) with (subst_map uus ∘ Var) by done. 
-        iDestruct (subst_map_var Δ uus with "[HΔ]") as "(%uus' & %Hrwuus')". 
-        { rewrite /uus. rewrite -env_sem_typed_insert; last (by rewrite HΔeq).
-          by rewrite -env_sem_typed_difference_delete. }
-        rewrite Hrwuus'. 
-        rewrite (app_mult_cons (c u)).
-        rewrite Hcons.
-        iApply ewp_bind_app_mult.
-        iApply (ewp_mono with "[Hκb Hκ]").
-        { iApply ("Hκb" with "Hκ"). iNext.  iApply "IH". }
-        iIntros (u') "Hu' !> /=". rewrite -Hcons -app_mult_cons -Hrwuus'.
-        iSpecialize ("Hu'" $! #() uus).
-        rewrite /uus -env_sem_typed_insert; last (by rewrite HΔeq).
-        rewrite -env_sem_typed_difference_delete; last done. 
-        iApply (ewp_mono with "[HΔ Hu']").
-        { by iApply ("Hu'" with "HΔ"). }
-        iIntros (?) "[$ HΓ₃] !>". 
-        rewrite -(env_sem_typed_insert _ _ w); last done.
-        by rewrite -env_sem_typed_difference_delete; last (rewrite HΔeq).
+      iIntros "(%α & %a & <- & Ha & Hκb) //=". ewp_pure_steps.
+      rewrite decide_True; [|split; first done; by injection].
+      rewrite subst_subst_ne; last done.
+      rewrite -subst_map_insert -delete_insert_ne; last done.
+      rewrite -subst_map_insert.
+      iApply (ewp_pers_mono with "[HΓ' Hκb Ha]"); [iApply "Hhms"; solve_env|].
+      + iDestruct "Hκb" as "#Hκb".
+        iIntros "!# %b Hκ /=".
+        iApply (ewp_pers_mono with "[Hκ]"); [iApply ("Hκb" with "Hκ IH")|].
+        iIntros "!# % [Hτ' _] !> //=".
+      + by (do 2 (rewrite -env_sem_typed_insert; try done)).
+      + iIntros "!# %u [$ HΓ₃] !>".
+        rewrite -(env_sem_typed_insert _ _ w a); last done.
+        by rewrite -(env_sem_typed_insert _ _ k c).
+  Qed.
+
+  Lemma sem_typed_deep_try_os Γ₁ Γ₂ Γ₃ Γ' w k e h r A B τ τ' ρs `{NonExpansive2 A, NonExpansive2 B }:
+    w ∉ env_dom Γ₂ → w ∉ env_dom Γ' → k ∉ env_dom Γ' →
+    w ∉ env_dom Γ₃ → k ∉ env_dom Γ₃ → w ≠ k → copy_env Γ' →
+    let ρ := (∀μTS: θ, α, A α θ ⇒ B α θ)%R in
+    Γ₁ ⊨ e : ⟨ρ,⟩ : τ' ⊨ Γ₂ -∗
+    (∀ α, (w, A α ρ) :: (k, B α ρ -{ ρs }-∘ τ) :: Γ' ⊨ h : ρs : τ ⊨ Γ₃) -∗
+    (w, τ') :: Γ₂ ++ Γ' ⊨ r : ρs : τ ⊨ Γ₃ -∗
+    Γ₁ ++ Γ' ⊨ (deep-try-dual: e
+                  effect  (λ: w k, h) 
+                | effectₘ (λ: w k, w) 
+                | return  (λ: w, r) end) : ρs : τ ⊨ Γ₃.
+  Proof.
+    iIntros (???????) "%ρ #He #Hh #Hr".
+    set Bot := (λ (_ : sem_ty Σ) (_ : sem_sig Σ), @sem_ty_void Σ).
+    iApply (sem_typed_deep_try _ Γ₂ _ _ _ _ _ _ _ _ A B Bot Bot with "[] [Hh] [] [Hr]"); try assumption.
+    - iApply sem_typed_sub_sig; [|iApply "He"]. rewrite /ρ.
+      apply sigs_le_comp; [apply sig_le_refl|apply sig_le_nil].
+    - simpl. rewrite /ρ. iIntros (α).
+      iApply sem_typed_sub_env; [|iApply "Hh"].
+      apply env_le_cons; [|apply ty_le_refl].
+      apply env_le_cons; [apply env_le_refl|].
+      apply ty_le_aarr; [|apply ty_le_refl|apply ty_le_refl].
+      apply sigs_le_refl.
+    - iIntros (α). rewrite /Bot /=. 
+      iApply sem_typed_sub_nil. iApply sem_typed_bot_in_env.
+    - iApply "Hr".
+  Qed.
+
+  Lemma sem_typed_deep_try_ms Γ₁ Γ₂ Γ₃ Γ' w k e h r A B τ τ' ρs `{NonExpansive2 A, NonExpansive2 B }:
+    w ∉ env_dom Γ₂ → w ∉ env_dom Γ' → k ∉ env_dom Γ' →
+    w ∉ env_dom Γ₃ → k ∉ env_dom Γ₃ → w ≠ k → copy_env Γ' →
+    let ρ := (∀μTSₘ: θ, α, A α θ ⇒ B α θ)%R in
+    Γ₁ ⊨ e : ⟨,ρ⟩ : τ' ⊨ Γ₂ -∗
+    (∀ α, (w, A α ρ) :: (k, B α ρ -{ ρs }-> τ) :: Γ' ⊨ h : ρs : τ ⊨ Γ₃) -∗
+    (w, τ') :: Γ₂ ++ Γ' ⊨ r : ρs : τ ⊨ Γ₃ -∗
+    Γ₁ ++ Γ' ⊨ (deep-try-dual: e
+                  effect  (λ: w k, w) 
+                | effectₘ (λ: w k, h) 
+                | return  (λ: w, r) end) : ρs : τ ⊨ Γ₃.
+  Proof.
+    iIntros (???????) "%ρ #He #Hh #Hr".
+    set Bot := (λ (_ : sem_ty Σ) (_ : sem_sig Σ), @sem_ty_void Σ).
+    iApply (sem_typed_deep_try _ Γ₂ _ _ _ _ _ _ _ _ Bot Bot A B with "[] [Hh] [] [Hr]"); try assumption.
+    - iApply sem_typed_sub_sig; [|iApply "He"]. rewrite /ρ.
+      apply sigs_le_comp; [apply sig_le_nil|apply sig_le_refl].
+    - iIntros (α). rewrite /Bot /=. 
+      iApply sem_typed_sub_nil. iApply sem_typed_bot_in_env.
+    - simpl. rewrite /ρ. iIntros (α).
+      iApply sem_typed_sub_env; [|iApply "Hh"].
+      apply env_le_cons; [|apply ty_le_refl].
+      apply env_le_cons; [apply env_le_refl|].
+      apply ty_le_uarr; [|apply ty_le_refl|apply ty_le_refl].
+      apply sigs_le_refl.
+    - iApply "Hr".
   Qed.
 
 End compatibility.
